separate projection functions from proof file
git-svn-id: https://scm.gforge.inria.fr/anonscm/svn/simsoc-cert@1790 ce709078-17db-4df8-89f4-d3e5bb8270d9

devel/xiaomu/test_csem_draft.v
@@ -1,753 +1,29 @@
-(* This file describe the relation between COQ and C state for ARM *)
-
 Require Import Globalenvs Memory.
 Require Import Csyntax Csem Cstrategy Coqlib Integers Values Maps Errors. 
 Require Import Arm6_State Arm6_Proc Arm6_SCC Bitvec Arm6.
 Require Import adc_compcert_fixed.
-
-(* Some constants for ADC *)
-
-(* Initial local environment, an empty PTree contents var location & type*)
-Definition env0 := (PTree.empty (block * type)).
-
-(* Initialize the memory with program p defined in adc_compcert*)
-Definition mem0 := Genv.init_mem p. 
-
-(* If an option val is Some integer then return the integer value else return zero*)
-Definition load_val (v : option val):word:=
-  match v with
-    |Some (Vint v')=> v'                     
-    |_ => Int.zero
-  end.
-
-(* Find the offset for elements in a struct*)
-(* If there is no variable id in struct t then the returned offset will be zero
-   (this location is then the same as for t);
-   later, if you want to L/S a value from this location, it will return None
- *)
-
-Definition ofs_of_fld (f_id:AST.ident) (fl:fieldlist) :word:=
-  match field_offset f_id fl with
-    | Error _ => Int.zero
-    | OK r => repr r
-  end.
-
-(* offset of each element in Processor Tstruct *)
-Definition cpsr_ofs:int:=ofs_of_fld cpsr typ_struct_SLv6_Processor.
-
-Definition spsr_ofs:int:=ofs_of_fld spsrs typ_struct_SLv6_Processor.
-
-Definition mode_ofs:int:=
-  add (ofs_of_fld cpsr typ_struct_SLv6_Processor) 
-  (ofs_of_fld mode typ_struct_SLv6_StatusRegister).
-
-Definition reg_ofs (id:AST.ident):int:=
-  ofs_of_fld id typ_struct_SLv6_Processor.
-
-Definition mmu_ofs:int:=ofs_of_fld mmu_ptr typ_struct_SLv6_Processor.
-
-Definition mem_ofs:int:=ofs_of_fld mem typ_struct_SLv6_MMU.
-
-Definition cp15_ofs:int:=ofs_of_fld cp15 typ_struct_SLv6_Processor.
-
-Definition pc_ofs:int:=ofs_of_fld pc typ_struct_SLv6_Processor.
-
-Definition id_ofs:int:=ofs_of_fld id typ_struct_SLv6_Processor.
-
-Definition jump_ofs:int:=ofs_of_fld jump typ_struct_SLv6_Processor.
-
-Definition proc_loc (m:Mem.mem) (e:env):option val:=
-  match e!proc with
-    |Some(b,_)=>
-      match 
-        (load_value_of_type (Tpointer typ_SLv6_Processor) m b Int.zero) with
-        |Some(Vptr b o) as v=>v
-        |_=>None
-      end
-    |None=>None
-  end.
-
-
-(* Projection from C parameters to COQ parameters*)
-(* If in local env the parameter of ADC (S, cond, d or n) exists,
-   then return the value of it else return zero*)
-
-Definition param_val (id:AST.ident) (m:Mem.mem) (e:env):val:=
-  match e!id with
-    |Some(b,t)=>
-      let ov:=load_value_of_type t m b Int.zero in
-        match ov with
-          |Some v=>v
-          |None=>Vundef
-        end
-    |None=>Vundef
-  end.
-
-Definition varg_proj (v:val):int:=
-  match v with
-    |Vint v'=>v'
-    |_=>Int.zero
-  end.
-
-Definition S_proj (m:Mem.mem) (e:env):bool:=
-  eq (varg_proj (param_val S m e)) w1.
-
-Definition cond_proj (m:Mem.mem) (e:env):opcode:= 
-  let c:=condition (varg_proj (param_val cond m e)) in
-    match c with
-      |Some c'=>c'
-      |None=>AL
-    end.
-
-Definition d_proj (m:Mem.mem) (e:env):regnum:=
-  mk_regnum (varg_proj (param_val d m e)).
-
-Definition n_proj (m:Mem.mem) (e:env):regnum:=
-  mk_regnum (varg_proj (param_val n m e)).
-
-Definition so_proj (m:Mem.mem) (e:env):word:=
-  varg_proj (param_val shifter_operand m e).
-
-Definition find_field (ofs:int) (m:Mem.mem) (e:env)
-  :option val:=
-  match proc_loc m e with
-    |Some(Vptr b o) => Some (Vptr b (add o ofs))
-    |_=>None
-  end.
-
-Definition find_cpsr (m:Mem.mem) (e:env):option val:=
-  find_field cpsr_ofs m e.
-
-Definition find_spsr (m:Mem.mem) (e:env):option val:=
-  find_field spsr_ofs m e.
-
-Definition find_reg (m:Mem.mem) (e:env) (rid:AST.ident):option val:=
-  find_field (ofs_of_fld rid typ_struct_SLv6_Processor) m e.
-
-Definition find_cp15 (m:Mem.mem) (e:env):option val:=
-  find_field cp15_ofs m e.
-
-Definition find_id (m:Mem.mem) (e:env):option val:=
-  find_field id_ofs m e.
-
-Definition find_jump (m:Mem.mem) (e:env):option val:=
-  find_field jump_ofs m e.
-
-(* If cpsr can be found, use the location of [cpsr] and the offset of 
-   mode in StatusRegister struct to get location of [mode]*)
-(* The mode field in cpsr and spsr should be the same. 
-   And the element of spsrs array which is in use should correspond to the same mode.
-   And the register array in use, should also corresponds to this mode.*)
-Definition find_mode (m:Mem.mem) (e:env):option val:=
-  match find_cpsr m e with
-    |Some(Vptr b ofs)=>Some(Vptr b (add ofs mode_ofs))
-    |_=>None
-  end.
-
-(* If in local environment the variable [porc] exists,
-   then return the pointer of [proc] field [mmu_ptr].
-   From this MMU struct, returns the pointer to the field [mem]*)
-Definition find_mmu (m:Mem.mem) (e:env):option val:=
-  match proc_loc m e with
-    |Some(Vptr bp op)=>
-      match 
-        (load_value_of_type (Tpointer typ_SLv6_MMU) m bp (add op mmu_ofs)) with
-        |Some(Vptr bm om) as v=>v
-        |_=>None
-      end
-    |_=>None
-  end.
-
-Definition find_mem (m:Mem.mem) (e:env):option val:=
-  match find_mmu m e with
-    |Some(Vptr bm om)=>
-      match 
-        (load_value_of_type (Tpointer(Tint I8 Unsigned)) m bm (add om mem_ofs)) with
-        |Some(Vptr b o) as v=>v
-        |_=>None
-      end
-    |_=>None
-  end.
-
-(* If in local environment the variable [proc] exists
-   then return the pointer of [proc] field [pc]*)
-(* the pointer to [pc] should point to the exact location of
-   the 16th element in array [user_regs]*)
-Definition find_pc (m:Mem.mem) (e:env):option val:=
-  match proc_loc m e with
-    |Some(Vptr b ofs)=>
-      match 
-        (load_value_of_type (Tpointer (Tint I32 Unsigned)) m b ofs) with
-        |Some(Vptr b o) as v=>v
-        |_=>None
-      end
-    |_=>None
-  end.
-
-Definition pc_usereg15 (m:Mem.mem) (e:env):Prop:=
-  find_pc m e = find_reg m e user_regs.
-
-Definition find_fld (f: Mem.mem->env->option val) (fld:fieldlist)
-  (id:AST.ident) (m:Mem.mem) (e:env):
-  option val:=
-  match f m e with
-    |Some(Vptr bp op)=> 
-      Some(Vptr bp (add op (ofs_of_fld id fld)))
-    |_=>None
-  end.
-
-(*
-(*memory blocks of SystemCoproc*)
-(*Record sc_mem := mk_scm
-  {eeb: option val;
-    ub: option val;
-    vb: option val}.
-*)
-Record sc_mem := mk_scm
-  {eeb: val;
-    ub: val;
-    vb: val}.
-
-Definition slv6_sc (m:Mem.mem) (e:env):option sc_mem:=
-  let fld_v b o id:= Vptr b (add o (ofs_of_fld id typ_struct_SLv6_SystemCoproc))
-    in
-    match find_cp15 m e with
-      |Some(Vptr b o)=> 
-        Some(mk_scm (fld_v b o ee_bit) (fld_v b o u_bit) (fld_v b o v_bit))
-      |_=>None
-  end.
-
-(*memory blocks of StatusRegister*)
-(*Record sr_mem := mk_srm
-  {nf: option val;
-    zf: option val;
-    cf: option val;
-    vf: option val;
-    qf: option val;
-    jf: option val;
-    ge0: option val;
-    ge1: option val;
-    ge2: option val;
-    ge3: option val;
-    ef: option val;
-    af: option val;
-    i_f: option val;
-    ff: option val;
-    tf: option val;
-    md: option val;
-    bg: option val}.
-*)
-Record sr_mem := mk_srm
-  {nf: val;
-    zf: val;
-    cf: val;
-    vf: val;
-    qf: val;
-    jf: val;
-    ge0: val;
-    ge1: val;
-    ge2: val;
-    ge3: val;
-    ef: val;
-    af: val;
-    i_f: val;
-    ff: val;
-    tf: val;
-    md: val;
-    bg: val}.
-
-Definition slv6_cpsr (m:Mem.mem) (e:env):option sr_mem:=
-  let fld_v b o id:=Vptr b (add o (ofs_of_fld id typ_struct_SLv6_StatusRegister))
-    in
-    match find_cpsr m e with
-      |Some(Vptr b o)=>
-        Some(mk_srm (fld_v b o N_flag) (fld_v b o Z_flag) (fld_v b o C_flag) 
-          (fld_v b o V_flag) (fld_v b o Q_flag) (fld_v b o J_flag) 
-          (fld_v b o GE0) (fld_v b o GE1) (fld_v b o GE2) (fld_v b o GE3)
-          (fld_v b o E_flag) (fld_v b o A_flag) (fld_v b o I_flag) 
-          (fld_v b o F_flag) (fld_v b o T_flag) (fld_v b o mode) 
-          (fld_v b o background))
-    |_=>None
-    end.
-
-Definition mode2mode (pm:proc_mode) :=
-  match pm with
-    |usr|sys=>(user_regs,5)
-    |exn e=>match e with
-              |fiq=>(fiq_regs,0)
-              |irq=>(irq_regs,1)
-              |svc=>(svc_regs,2)
-              |abt=>(abt_regs,3)
-              |und=>(und_regs,4)
-            end
-  end.
-
-(*Definition find_spsr_m (m:Mem.mem) (e:env) (em:exn_mode):option val:=
-  let ofs o :=
-    add o (repr ((snd (mode2mode (exn em)))*sizeof typ_SLv6_StatusRegister)) in
-  match find_spsr m e with
-    |Some(Vptr b o)=>
-      Some (Vptr b (ofs o))
-    |_=>None
-  end.
-*)
-Definition find_spsr_m (m:Mem.mem) (e:env):option(exn_mode->val):=
-  let ofs o em:=
-    add o (repr ((snd (mode2mode (exn em)))*sizeof typ_SLv6_StatusRegister)) in
-  match find_spsr m e with
-    |Some(Vptr b o)=>
-      Some(fun em=>(Vptr b (ofs o em)))
-    |_=>None
-  end.
-
-Definition blk_spsr (m:Mem.mem) (e:env):=
-  let ofs o em:=
-    add o (repr ((snd (mode2mode (exn em)))*sizeof typ_SLv6_StatusRegister)) in
-  match find_spsr m e with
-    |Some(Vptr b o)=>
-      Some(fun em=>(b, (ofs o em)))
-    |_=>None
-  end.
-
-Definition slv6_spsr (m:Mem.mem) (e:env):option(exn_mode->sr_mem):=
-  let fld_v b o id:=Vptr b (add o (ofs_of_fld id typ_struct_SLv6_StatusRegister))
-    in
-    match blk_spsr m e with
-      |Some v=>
-        Some(fun em=>let (b,o):=v em in 
-          mk_srm (fld_v b o N_flag) (fld_v b o Z_flag) (fld_v b o C_flag) 
-          (fld_v b o V_flag) (fld_v b o Q_flag) (fld_v b o J_flag) 
-          (fld_v b o GE0) (fld_v b o GE1) (fld_v b o GE2) (fld_v b o GE3)
-          (fld_v b o E_flag) (fld_v b o A_flag) (fld_v b o I_flag) 
-          (fld_v b o F_flag) (fld_v b o T_flag) (fld_v b o mode) 
-          (fld_v b o background))
-      |_=>None
-    end.
-
-(*memory blocks of MMU*)
-Record mmu_mem := mk_mmum
-  {bgn: val;
-    sz: val;
-    ed: val;
-    mm: val}.
-
-(*Record mmu_mem := mk_mmum
-  {bgn: option val;
-    sz: option val;
-    ed: option val;
-    mm: option val}.
-*)
-
-Definition slv6_mmu (m:Mem.mem) (e:env):option mmu_mem:=
-  let fld_v b o id:=Vptr b (add o (ofs_of_fld id typ_struct_SLv6_MMU)) in
-  match find_mmu m e with
-    |Some(Vptr b o)=>
-      Some(mk_mmum (fld_v b o begin) (fld_v b o size) 
-                   (fld_v b o _end) (fld_v b o mem))
-    |_=>None
-  end.
-
-(*memory blocks of proc*)
-Record proc_mem := mk_pcm
-  {mmup: mmu_mem;
-    cpsr_m: sr_mem;
-    spsr_m: exn_mode->sr_mem;
-    sc: sc_mem;
-    id: val;
-    rg: register->val;
-    p: val;
-    jp: val}.
-
-Definition reg2reg (r:register):=
-  match r with
-    |R k=>(user_regs,k)
-    |R_svc k _=>(svc_regs,mk_regnum k)
-    |R_abt k _=>(abt_regs,mk_regnum k)
-    |R_und k _=>(und_regs,mk_regnum k)
-    |R_irq k _=>(irq_regs,mk_regnum k)
-    |R_fiq k _=>(fiq_regs,mk_regnum k)
-  end.
-
-Definition slv6_proc (m:Mem.mem) (e:env):option proc_mem:=
-  let fld_v b o i:=Vptr b (add o (ofs_of_fld i typ_struct_SLv6_Processor)) in
-  let fld_reg b o r:=
-    Vptr b (add o (ofs_of_fld (fst(reg2reg r)) 
-      typ_struct_SLv6_Processor)) in
-  let mm:=slv6_mmu m e in
-  let c:=slv6_cpsr m e in
-  let s:=slv6_spsr m e in
-  let sc:=slv6_sc m e in
-    match proc_loc m e with
-      |Some(Vptr b o)=>
-        match mm,c,(*fs,is,ss,abs,us,*)s,sc with
-          |Some vm,Some vc,(*Some vfs,Some vis,Some vss,Some vabs,Some vus,*)
-            Some vs,Some vsc =>
-            Some(mk_pcm vm vc (*vfs vis vss vabs vus*) vs vsc 
-              (fld_v b o adc_compcert_fixed.id) 
-              (fld_reg b o)
-              (fld_v b o pc)
-              (fld_v b o jump))
-          |_,_,_,_(*,_,_,_,_*)=>None
-        end
-      |_=>None
-    end.
-
-(* From a StateRegister Tstruct to word*)
-Definition sr_proj (m:Mem.mem) (sr:sr_mem) :option word:=
-  let valof ptr typ :=
-    match ptr with
-      |Vptr b o=>load_value_of_type typ m b o
-      |_=>None
-    end in
-    let setcpsr n ov ow :=
-      match ov, ow with
-        |Some(Vint v), Some w=>Some (set_bit n v w)
-        |_,_=>None
-      end in 
-    let setcpsrs n1 n2 ov ow :=
-      match ov, ow with
-        |Some(Vint v), Some w=>Some (set_bits n1 n2 v w)
-        |_,_=>None
-      end in 
-    (setcpsr Nbit (valof sr.(nf) (Tint I8 Unsigned))
-    (setcpsr Zbit (valof sr.(zf) (Tint I8 Unsigned))
-    (setcpsr Cbit (valof sr.(cf) (Tint I8 Unsigned))
-    (setcpsr Vbit (valof sr.(vf) (Tint I8 Unsigned))
-    (setcpsr Qbit (valof sr.(qf) (Tint I8 Unsigned))
-    (setcpsr Jbit (valof sr.(jf) (Tint I8 Unsigned))
-(* set bits 16 to 19 is set GEbits*)
-    (setcpsr 19%nat (valof sr.(ge3) (Tint I8 Unsigned))
-    (setcpsr 18%nat (valof sr.(ge2) (Tint I8 Unsigned))
-    (setcpsr 17%nat (valof sr.(ge1) (Tint I8 Unsigned))
-    (setcpsr 16%nat (valof sr.(ge0) (Tint I8 Unsigned))
-    (setcpsr Ebit (valof sr.(ef) (Tint I8 Unsigned))
-    (setcpsr Abit (valof sr.(af) (Tint I8 Unsigned))
-    (setcpsr Ibit (valof sr.(i_f) (Tint I8 Unsigned))
-    (setcpsr Fbit (valof sr.(ff) (Tint I8 Unsigned)) 
-    (setcpsr Tbit (valof sr.(tf) (Tint I8 Unsigned)) 
-(* set bits 0 to 4 is set Mbits*)
-    (setcpsrs 0%nat 4%nat (valof sr.(md) (Tint I32 Unsigned)) 
-      (Some Int.zero))))))))))))))))).
-
-(* Projection form C cpsr to COQ cpsr*)
-Definition cpsr_proj (m:Mem.mem) (c:sr_mem):option word:=
-  sr_proj m c.
-
-Definition spsr_proj (m:Mem.mem) (s:exn_mode->sr_mem) (em:exn_mode):word:=
-  let sr:=s em in
-    match sr_proj m sr with
-      |Some w=>w
-      |None=>repr 16
-    end.
-
-(* Projection from C mode in cpsr, to COQ mode*)
-Definition mode_proj (m:Mem.mem) (c:sr_mem) :option proc_mode:=
-  match c.(md) with
-    |Vptr b o=>
-      match load_value_of_type (Tint I32 Unsigned) m b o with
-        |Some(Vint v)=>proc_mode_of_word v
-        |_=>None
-      end
-    |_=>None
-  end.
-
-
-(* Projection from C reg to COQ reg*)
-Definition regs_proj (m:Mem.mem) (p:proc_mem) (r:register):word:=
-  let valof k:=
-    match p.(rg) r with
-      |Vptr b o=>load_value_of_type (Tint I32 Unsigned) m b (add o (repr k))
-      |_=>None
-    end in
-    let reg_val v :=
-    match v with
-      |Some(Vint v')=> v'
-      |_=>w0
-    end in
-    reg_val (valof (snd(reg2reg r))).
-
-
-(* Projection from C memory to COQ memory*)
-Definition mem_proj (m:Mem.mem) (mu:mmu_mem) (ad:address): word:=
-  match mu.(mm) with
-    |Vptr b o=>
-      match
-        load_value_of_type (Tint I8 Unsigned) m b (add o (word_of_address ad)) with
-        |Some(Vint v)=>v
-        |_=>w0
-      end
-    |_=>w0
-  end.
-
-(*Definition mem_proj (m:Mem.mem) (e:env) (ad:address):option word:=
-  match (find_mem m e) with
-    |Some(Vptr b o)=>
-      match load_value_of_type (Tint I8 Unsigned) m b 
-        (add o (word_of_address ad)) with
-        |Some(Vint v)=>Some v
-        |_=>None
-      end
-    |_=>None
-  end.*)
-
-(* Projection from C cp15 to COQ SCC register*)
-Definition screg_proj (m:Mem.mem) (sc:sc_mem) (r:regnum): word:=
-  let bit_val_e :=
-  match sc.(eeb) with
-    |Vptr b o=> load_value_of_type (Tint I8 Unsigned) m b o
-    |_=>None
-  end in
-  let bit_val_u :=
-  match sc.(ub) with
-    |Vptr b o=> load_value_of_type (Tint I8 Unsigned) m b o
-    |_=>None
-  end in
-  let bit_val_v :=
-  match sc.(vb) with
-    |Vptr b o=> load_value_of_type (Tint I8 Unsigned) m b o
-    |_=>None
-  end in  
-  let setscreg n ov ow :=
-    match ov, ow with
-      |Some(Vint v),w=>set_bit n v w
-      |_,_=>w0
-    end in
-    setscreg Vbit (bit_val_v) 
-    (setscreg Ubit (bit_val_u) 
-    (setscreg EEbit (bit_val_e) Int.zero)).  
-
-
-(* Projection from C proc to COQ state. exn in COQ proc state is assigned by
-   a nil exception list*)
-
-Definition proc_proj (m:Mem.mem) (e:env):option (Arm6_State.state):=
-  let mkpst ocpsr vspsr vreg omode:=
-    match ocpsr, omode with
-      |Some vcpsr, Some vmode=>
-        Some (Arm6_Proc.mk_state vcpsr vspsr vreg nil vmode)
-      |_,_ => None
-    end in
-    let mksst vscreg vmem := Arm6_SCC.mk_state vscreg vmem in
-      let mkst oproc vscc :=
-        match oproc with
-          |Some vproc=>Some (Arm6_State.mk_state vproc vscc)
-          |_=>None
-        end in
-        let opc := slv6_proc m e in
-        match opc with
-          |Some pc =>
-            mkst (mkpst (cpsr_proj m pc.(cpsr_m)) (spsr_proj m pc.(spsr_m)) 
-            (regs_proj m pc) 
-            (mode_proj m pc.(cpsr_m)))
-          (mksst (screg_proj m pc.(sc)) (mem_proj m pc.(mmup)))
-          |None=>None
-        end.
-*)
-
-
-(* From a StateRegister Tstruct to word*)
-(* Every bit is transformed from uint8 to one bit *)
-
-Definition fld_sr:= typ_struct_SLv6_StatusRegister.
-
-
-Definition sr_proj (m:Mem.mem) (b:block) (ofs:int) :word:=
-  let load_val_of id tp :=
-    load_val (load_value_of_type tp m b 
-      (add ofs (ofs_of_fld id fld_sr))) in
-  let nflag := load_val_of N_flag (Tint I8 Unsigned) in
-  let zflag := load_val_of Z_flag (Tint I8 Unsigned) in
-  let cflag := load_val_of C_flag (Tint I8 Unsigned) in
-  let vflag := load_val_of V_flag (Tint I8 Unsigned) in
-  let qflag := load_val_of Q_flag (Tint I8 Unsigned) in
-  let jflag := load_val_of J_flag (Tint I8 Unsigned) in
-  let ge0 := load_val_of GE0 (Tint I8 Unsigned) in
-  let ge1 := load_val_of GE1 (Tint I8 Unsigned) in
-  let ge2 := load_val_of GE2 (Tint I8 Unsigned) in
-  let ge3 := load_val_of GE3 (Tint I8 Unsigned) in
-  let eflag := load_val_of E_flag (Tint I8 Unsigned) in
-  let aflag := load_val_of A_flag (Tint I8 Unsigned) in
-  let iflag :=  load_val_of I_flag (Tint I8 Unsigned) in
-  let fflag := load_val_of F_flag (Tint I8 Unsigned) in
-  let tflag := load_val_of T_flag (Tint I8 Unsigned) in
-  let md := load_val_of mode (Tint I32 Unsigned) in
-(* according to P49,
-   Implementations must read reversed bits as 0 and ignore writes to them.
-   So no setting bits for the reversed bits*)
-  let bg := Int.zero in
-    (set_bit Nbit nflag
-    (set_bit Zbit zflag
-    (set_bit Cbit cflag
-    (set_bit Vbit vflag
-    (set_bit Qbit qflag
-    (set_bit Jbit jflag
-(* set bits 16 to 19 is set GEbits*)
-    (set_bit 19 ge3
-    (set_bit 18 ge2
-    (set_bit 17 ge1
-    (set_bit 16 ge0
-    (set_bit Ebit eflag
-    (set_bit Abit aflag
-    (set_bit Ibit iflag 
-    (set_bit Fbit fflag 
-    (set_bit Tbit tflag 
-(* set bits 0 to 4 is set Mbits*)
-    (set_bits 4 0 md Int.zero)))))))))))))))).
-
-(* Projection form C cpsr to COQ cpsr*)
-(* If the location of cpsr is found, then project C cpsr to a word
-   else return zero*)
-Definition cpsr_proj (m:Mem.mem) (e:env) :word:=
-  match find_cpsr m e with
-    |Some (Vptr b ofs) => sr_proj m b ofs
-    |_ => Int.zero
-  end.
-
-(* Projection from C spsr to COQ spsr*)
-(* If the location of spsr of specified exception mode is found, 
-   then project C cpsr to a word else return zero*)
-Definition spsr_proj (m:Mem.mem) (e:env) (em:exn_mode):word:=
-  let ofs o n:=add o (repr (n*sizeof typ_SLv6_StatusRegister)) in
-  match find_spsr m e with
-    |Some(Vptr b o)=>
-      match em with
-        |fiq=>sr_proj m b (ofs o 0)
-        |irq=>sr_proj m b (ofs o 1)
-        |svc=>sr_proj m b (ofs o 2)
-        |abt=>sr_proj m b (ofs o 3)
-        |und=>sr_proj m b (ofs o 4)
-      end
-    |_=>Int.zero
-  end.
-
-(* Projection from C mode in cpsr, to COQ mode*)
-(* If the location of mode is found, 
-   then project C mode to a proc_mode else return default user mode*)
-(* The mode in cpsr should indecate which spsr mode is and which kind of register
-   is used*)
-Definition mode_proj (m:Mem.mem) (e:env) :proc_mode:=
-  let om:=match find_mode m e with
-    |Some(Vptr b ofs)=>
-      proc_mode_of_word (load_val 
-        (load_value_of_type (Tint I32 Unsigned) m b ofs))
-    |_=>None
-  end
-  in 
-  match om with
-    |Some md=>md
-    |None=>usr
-  end.
-
-(* Projection from C reg to COQ reg*)
-(* If the location of reg is found, and by knowing which register mode
-   and which register number it is, return the value of this register.
-   else return zero*)
-Definition regs_proj (m:Mem.mem) (e:env) (r:register):word:=
-  let load_reg id n m e:=
-    match find_reg m e id with 
-    |Some(Vptr b ofs)=>
-      load_val (load_value_of_type 
-        (Tint I32 Unsigned) m b (add ofs (repr n))) 
-    |_=>Int.zero
-  end
-    in
-  match r with
-    | R k => load_reg user_regs k m e
-    | R_svc k _=> load_reg svc_regs k m e
-    | R_abt k _=> load_reg abt_regs k m e
-    | R_und k _=> load_reg und_regs k m e
-    | R_irq k _=> load_reg irq_regs k m e
-    | R_fiq k _=> load_reg fiq_regs k m e
-  end.
-
-(* Projection from C memory to COQ memory*)
-(* If the location of memory is found, using the address to
-   get the content of such memory block, else return zero*)
-Definition mem_proj (m:Mem.mem) (e:env) (ad:address):word:=
-  match find_mem m e with
-    |Some(Vptr b ofs)=>
-      load_val (load_value_of_type 
-        (Tint I8 Unsigned) m b (add ofs (word_of_address ad)))
-    |_=>Int.zero
-  end.
-
-(* Projection from C cp15 to COQ SCC register*)
-(* If the location of cp15 is found, 
-   get the value of ee_bit u_bit and v_bit to set the bits in
-   COQ SCC reg*)
-
-Definition fld_sc :=typ_struct_SLv6_SystemCoproc.
-
-Definition screg_proj (m:Mem.mem) (e:env) (r:regnum):word:=
-  match find_cp15 m e with
-    |Some(Vptr b ofs)=>
-      let regbit id:=
-        load_val (load_value_of_type (Tint I8 Unsigned) m b
-        (add ofs (ofs_of_fld id fld_sc))) in
-        let ee := regbit ee_bit in
-        let u := regbit u_bit in
-        let v := regbit v_bit in
-        set_bit Vbit v (set_bit Ubit u (set_bit EEbit ee Int.zero))
-    |_=>Int.zero
-  end.
-
-(* Projection from C proc to COQ state. exn in COQ proc state is assigned by
-   a nil exception list*)
-Definition proc_proj (m:Mem.mem) (e:env):Arm6_State.state:=
-  Arm6_State.mk_state 
-  (Arm6_Proc.mk_state (cpsr_proj m e) (spsr_proj m e) (regs_proj m e) nil (mode_proj m e))
-  (Arm6_SCC.mk_state (screg_proj m e) (mem_proj m e)).
-
-
-(* Stating theorems *)
+Require Import projection. 
 
 Require Import Arm6_Simul.
 Import I.
 Import Arm6_Functions.Semantics.
 
-Check proc_proj.
-
-(*Inductive proc_state_related : Mem.mem -> env -> @result unit -> Prop :=
-  |proc_state_related_ok : 
-    forall m e l b v, 
-      proc_proj m e = Some v ->
-      proc_state_related m e (Ok tt (mk_semstate l b v))
-  |state_not_ok: 
-    forall e m mes,
-      proc_proj m e = None ->
-      proc_state_related m e (Ko mes)
-  |state_todo: 
-    forall e m mes,
-      proc_proj m e = None ->
-      proc_state_related m e (Todo mes).*)
-
-Inductive proc_state_related : Mem.mem -> env -> @result unit -> Prop :=
-  |proc_state_related_ok : 
-    forall m e l b, proc_state_related m e (Ok tt (mk_semstate l b (proc_proj m e)))
-  |state_not_ok: forall e m mes, proc_state_related m e (Ko mes)
-  |state_todo: forall e m mes, proc_state_related m e (Todo mes).
-
-(* Functional relation between the C memory module which contains proc, 
-   and the COQ specification of Arm6 state *)
-(*Definition proc_state_func_related (m:Mem.mem) (e:env) (s:Arm6_State.state) :Prop:=
-  proc_proj m e = s.*)
-
 (* Functional relation between the C memory module which contains the other ADC parameters, 
    and the COQ specification of ADC parameters *)
 Definition sbit_func_related (m:Mem.mem) (e:env) (sbit:bool):Prop:=
-  S_proj m e = sbit.
+  bit_proj m e S = sbit.
 
 Definition cond_func_related (m:Mem.mem) (e:env) (cond:opcode):Prop:=
   cond_proj m e = cond.
 
 Definition d_func_related (m:Mem.mem) (e:env) (d:regnum):Prop:=
-  d_proj m e = d.
+  reg_proj m e adc_compcert_fixed.d = d.
 
 Definition n_func_related (m:Mem.mem) (e:env) (n:regnum):Prop:=
-  n_proj m e = n.
+  reg_proj m e adc_compcert_fixed.n = n.
 
 Definition so_func_related (m:Mem.mem) (e:env) (so:word):Prop:=
-  so_proj m e = so.
+  bits_proj m e shifter_operand = so.
 
 (* Human readable renaming of [p], which is generated by the Coq printer *)
 (*Definition prog_adc := adc_compcert_fixed.p.*)
@@ -794,6 +70,7 @@ Ltac nod :=
 Parameter of_mem : AST.ident -> Mem.mem -> Mem.mem.
 
 (*exp get_bit*)
+Print fun_internal_ADC.
 
 Definition reg_id id :=
   Ecall (Evalof (Evar reg T2) T2)
@@ -801,13 +78,13 @@ Definition reg_id id :=
     (Econs 
       (Evalof (Evar id T4) T4) Enil)) T1.
 
-Definition get_bit_reg :=
+Definition get_rd_bit31 :=
   Ecall (Evalof (Evar get_bit T16) T16)
   (Econs (reg_id d)
     (Econs (Eval (Vint (repr 31)) T9)
       Enil)) T4.
 
-Lemma get_rg_ok :
+Lemma same_reg_d :
   forall e m t m' a' l b st d,
     proc_state_related m e (Ok tt (mk_semstate l b st)) ->
     d_func_related m e d ->    
@@ -817,60 +94,6 @@ Lemma get_rg_ok :
 Admitted.
 
 Set Implicit Arguments.
-
-Lemma alloc_diff_block' :
-  forall m e e' m' x y b_x tx b_y ty vlst,
-    alloc_variables e m ((x,tx)::(y,ty)::vlst) e' m'->
-    list_norepet (x::y::var_names vlst) ->
-    e' ! x = Some (b_x, tx) ->
-    e' ! y = Some (b_y, ty) ->
-    b_x <> b_y.
-Proof.
-  intros until vlst. intros av norepet getx gety.
-  inv av. inv H7.
-  apply Mem.valid_new_block in H6.
-  unfold Mem.valid_block in H6.
-  apply Mem.alloc_result in H8.
-  rewrite <- H8 in H6; clear H8.
-  apply Zlt_not_eq in H6.
-  induction vlst.
-    inv H9. 
-    assert (findy: (PTree.set y (b0, ty) (PTree.set x (b1, tx) e)) ! y =
-           Some (b0, ty)).
-    apply PTree.gss. rewrite findy in gety. inversion gety.
-    assert (findx: (PTree.set y (b0, ty) (PTree.set x (b1, tx) e)) ! x =
-           (PTree.set x (b1, tx) e) ! x).
-    apply PTree.gso.
-    inv norepet. unfold In in H2. intro exy. apply H2. left. symmetry. 
-    exact exy.
-    rewrite findx in getx.
-    rewrite PTree.gss in getx. inversion getx.
-    rewrite <- H0. rewrite <- H1.
-    exact H6. 
-(*
-    inv H9. inv H7. admit.
-    assert (findy: (PTree.set y (b0, ty) (PTree.set x (b1, tx) e)) ! y =
-           Some (b0, ty)).
-    apply PTree.gss. 
-    rewrite PTree.gso in gety;
-      [idtac | 
-        inv norepet; inv H2; unfold In in H4; intro eqyid0; apply H4; 
-    left; symmetry; exact eqyid0;
-    rewrite findy in gety; inversion gety].
-    rewrite findy in gety. inversion gety.
-
-    assert (findx: (PTree.set y (b0, ty) (PTree.set x (b1, tx) e)) ! x =
-           (PTree.set x (b1, tx) e) ! x).
-    apply PTree.gso.
-    inv norepet. unfold In in H2. intro exy. apply H2. 
-    left. symmetry. exact exy.
-*)    
-
- 
-    
-
-
-Admitted.
 
 Lemma alloc_diff_block :
   forall m e e' m' x y b_x tx b_y ty,
@@ -926,10 +149,11 @@ Proof.
   apply zero_ext_and with (x := (and (shru x (repr n)) (repr 1))) in H0.
   rewrite H0.  
   unfold bit. unfold bits. unfold bits_val.
-  unfold masks. SearchAbout minus. 
-  rewrite minus_diag. Print masks_aux.
+  unfold masks. (*SearchAbout minus. *)
+  rewrite minus_diag. (*Print masks_aux.*)
   simpl masks_aux. 
-  SearchAbout repr. rewrite shru_div_two_p.
+  (*SearchAbout repr.*)
+  rewrite shru_div_two_p.
 
 (*
   induction n. 
@@ -1176,16 +400,14 @@ Definition inv_expr_ecall' g e m ex m' ex':=
   end.
 
 
-
-
-Lemma same_nflag_assgnt' :
+Lemma same_get_reg' :
   forall e m0 m0' vargs m l b s d t m' v,
     alloc_variables empty_env m0 
       (fun_internal_ADC.(fn_params) ++ fun_internal_ADC.(fn_vars)) e m0' ->
     bind_parameters e m0' fun_internal_ADC.(fn_params) vargs m ->
     proc_state_related m e (Ok tt (mk_semstate l b s)) ->
     d_func_related m e d ->
-    eval_expression (Genv.globalenv prog_adc) e m get_bit_reg t m' v->
+    eval_expression (Genv.globalenv prog_adc) e m get_rd_bit31  t m' v->
     v = Vint ((Arm6_State.reg_content s d) [n31]).
 Proof.
   intros until v. intros av bp psrel dfrel get_bit.
@@ -1193,7 +415,7 @@ Proof.
   inversion get_bit as [env m1 gb t1 m1' gb' v1 gb_expr ev_rv Heqenv Heqm
     Heqexp Heqt Heqm' Heqv]; clear get_bit; subst.
 
-  unfold get_bit_reg in gb_expr.
+  unfold get_rd_bit31 in gb_expr.
 
 (*  revert ev_rv.
 *)
@@ -1420,14 +642,14 @@ Admitted.
 
 
 
-Lemma same_nflag_assgnt :
+Lemma same_get_reg :
   forall e m0 m0' vargs m l b s d t m' v,
     alloc_variables empty_env m0 
       (fun_internal_ADC.(fn_params) ++ fun_internal_ADC.(fn_vars)) e m0' ->
     bind_parameters e m0' fun_internal_ADC.(fn_params) vargs m ->
     proc_state_related m e (Ok tt (mk_semstate l b s)) ->
     d_func_related m e d ->
-    eval_expression (Genv.globalenv prog_adc) e m get_bit_reg t m' v->
+    eval_expression (Genv.globalenv prog_adc) e m get_rd_bit31 t m' v->
     v = Vint ((Arm6_State.reg_content s d) [n31]).
 Proof.
   intros until v. intros av bp psrel dfrel get_bit.
@@ -1441,7 +663,7 @@ Proof.
 
 
 
-  apply get_rg_ok with e m2 t1 m1 a1' l b s d in H4;
+  apply same_reg_d with e m2 t1 m1 a1' l b s d in H4;
     [idtac| exact psrel |exact dfrel].
   rewrite H4 in *. 
   inv H13. inv H5. inv H14.
@@ -1593,7 +815,6 @@ Axiom funct_unpredictable:
     (unpredictable Arm6_Message.EmptyMessage semstt).
 
 (* Assume function reg_n only load from memory, not change it*)
-
 Axiom get_reg_ok :
   forall e id m t m' r,
     eval_expr (Genv.globalenv prog_adc) e m RV (reg_id id) t m' r ->
@@ -1626,11 +847,13 @@ Qed.
 
 (* Lemmas on if ConditionPassed*)
 Definition condpass :=
-  Ecall (Evalof (Evar ConditionPassed T5) T5)
-  (Econs
-    (Eaddrof
-      (Efield (Ederef (Evalof (Evar proc T3) T3) T6) cpsr
-        T6) T6) (Econs (Evalof (Evar cond T7) T7) Enil)) T5.
+  (Ecall (Evalof (Evar ConditionPassed T5) T5)
+    (Econs
+      (Eaddrof
+        (Efield (Ederef (Evalof (Evar proc T3) T3) T6) cpsr
+          T7) T8)
+      (Econs (Evalof (Evar adc_compcert_fixed.cond T9) T9)
+        Enil)) T4).
 
 Axiom no_effect_condpass :
   forall e m m' t v,
@@ -1638,28 +861,66 @@ Axiom no_effect_condpass :
     m = m'/\eval_expression (Genv.globalenv prog_adc) e m condpass t m' v.
 
 Lemma condpass_false :
-  forall e m t m' v cond s,
+  forall m0 m0' e m t m' v cond s,
+    alloc_variables empty_env m0 
+      (fun_internal_ADC.(fn_params) ++ fun_internal_ADC.(fn_vars)) e m0' ->
     eval_expression (Genv.globalenv prog_adc) e m condpass t m' v ->
-    Csem.is_false v T5 ->
+    Csem.is_false v T4 ->
     Arm6_Functions.State.ConditionPassed s cond = false.
 Proof.
-  intros until s. intros cdps cdps_false.
+  intros until s. intros av cdps cdps_false.
   inv cdps_false.
+  inv cdps. inv H. inv H0.
+  inv H4. inv H3. inv H5. inv H3. inv H4. inv H14. inv H3. inv H4. inv H13.
+  inv H3. inv H4. inv H10.
+  inv H6.
+  inv av. inv H14. inv H17. inv H18. inv H19. inv H20. inv H21. inv H22.
+  pose (e:=
+    (PTree.set old_Rn (b6, Tint I32 Unsigned)
+      (PTree.set shifter_operand (b5, Tint I32 Unsigned)
+        (PTree.set n (b4, Tint I8 Unsigned)
+          (PTree.set d (b3, Tint I8 Unsigned)
+            (PTree.set adc_compcert_fixed.cond 
+              (b2, Tint I32 Signed)
+              (PTree.set S (b0, Tint I8 Unsigned)
+                (PTree.set proc (b1, Tpointer typ_SLv6_Processor)
+                  empty_env)))))))).
+  fold e in H7, H1.
+  inv H1. unfold e in H6; simpl in H6; discriminate H6.
+  inv H5. inv H10.
+  (*to be improve *)
 Qed.
 
 Lemma condpass_true :
-  forall e m t m' v cond s,
+  forall m0 m0' e m t m' v cond s,
+    alloc_variables empty_env m0 
+      (fun_internal_ADC.(fn_params) ++ fun_internal_ADC.(fn_vars)) e m0' ->
     eval_expression (Genv.globalenv prog_adc) e m condpass t m' v ->
-    Csem.is_true v T5 ->
+    Csem.is_true v T4 ->
     Arm6_Functions.State.ConditionPassed s cond = true.
 Proof.
-  intros until s. intros cdps cdps_true.
-  inv cdps_true.
+  intros until s. intros av cdps cdps_true.
+  inv cdps. inv H. inv H4. inv H9. inv H5. inv H4. inv H5. inv H15. inv H4.
+  inv H5. inv H14. inv H4. inv H5. inv H13.
+  inv H0. inv H6.
+  inv av. inv H14. inv H17. inv H18. inv H19. inv H20. inv H21. inv H22.
+  pose (e:=
+    (PTree.set old_Rn (b6, Tint I32 Unsigned)
+      (PTree.set shifter_operand (b5, Tint I32 Unsigned)
+        (PTree.set n (b4, Tint I8 Unsigned)
+          (PTree.set d (b3, Tint I8 Unsigned)
+            (PTree.set adc_compcert_fixed.cond 
+              (b2, Tint I32 Signed)
+                        (PTree.set S (b0, Tint I8 Unsigned)
+                          (PTree.set proc (b1, Tpointer typ_SLv6_Processor)
+                            empty_env)))))))).
+  fold e in H7, H1.
+  inv H1. unfold e in H6; simpl in H6; discriminate H6. inv H5. inv H10.
 Qed.
 
 (*Lemma on proc_state_relates holds after set_reg*)
 Definition set_regpc :=
-  Ecall (Evalof (Evar set_reg_or_pc T8) T8)
+  Ecall (Evalof (Evar set_reg_or_pc T10) T10)
   (Econs (Evalof (Evar proc T3) T3)
     (Econs (Evalof (Evar d T4) T4)
       (Econs
@@ -1673,21 +934,8 @@ Definition set_regpc :=
               (Efield
                 (Ederef
                   (Evalof (Evar proc T3) T3)
-                  (Tpointer T3)) cpsr T6)
-              C_flag T4) T4) T1) Enil))) T9.
-
-(*Axiom set_regpc_store :
-  forall m m' t v p_blk,
-    eval_expression (Genv.globalenv prog_adc) e m set_regpc t m' v ->
-    store_value_of_type T1 m p_blk (add (reg_ofs user_regs) (repr 15)) v = Some m'.
-
-Axiom set_regpc_ok:
-  forall m s0 s m' t v n so ,
-    eval_expression (Genv.globalenv prog_adc) e m set_regpc t m' v ->
-    mk_reg (R (mk_regnum 15)) 
-    (fun rn => (add (add (Arm6_State.reg_content s0 n) so)
-      (Arm6_State.cpsr s) [Cbit])) e (of_mem proc m) = (of_mem proc m').*)
-
+                  T6) cpsr T7) C_flag T4) T9)
+          T9) Enil))) T11.
 
 Lemma same_setregpc :
   forall e m l b s0 s t m' v d n so ,
@@ -1700,7 +948,10 @@ Lemma same_setregpc :
 Proof.
   intros until so. intros psrel setreg. intros.
   inv setreg. inv H. inv H4. inv H9. inv H5. inv H4. inv H5.
-  inv H14. inv H4. inv H5. inv H13. inv H4. inv H17. inv H15.
+  inv H14. inv H4. inv H5. inv H13. inv H4. inv H17. inv H15. inv H4.
+  inv H19. inv H4. inv H18. inv H4. inv H15. inv H13. inv H4. inv H5.
+  inv H14. inv H0.
+  (*inv H15.
   inv H4. inv H14. inv H19. inv H4. inv H18. inv H4. inv H14.
   inv H13. inv H4. inv H5.
   apply (functions_behavior_ok e l b s vf fd m2 vargs t3 m' vres l0 b0
@@ -1708,8 +959,8 @@ Proof.
       (add (add (Arm6_State.reg_content s0 n) so)
         (Arm6_State.cpsr s) [Cbit])))
     in psrel;
-    [apply psrel|exact H11|exact H16].
-Qed.
+    [apply psrel|exact H11|exact H16].*)
+Admitted.
 
 (* Lemmas on if S==1 *)
 Definition is_S_set :=
@@ -1736,7 +987,7 @@ Proof.
   inv s_set. inv H. inv H10. inv H4. inv H11.
   inv H0. inv H7.
   inv sfrel.
-  unfold S_proj.
+  unfold bit_proj.
   unfold param_val. inv H5. inv H6. inv H2. rewrite H6.
   rewrite H7. unfold varg_proj.
   destruct v1; try auto.
@@ -1758,7 +1009,7 @@ Proof.
   inv s_set. inv H. inv H10. inv H4. inv H11.
   inv H0. inv H6. inv H5. inv sfrel.
   simpl in H7.
-  unfold S_proj. unfold param_val. 
+  unfold bit_proj. unfold param_val. 
   inv H1.
     rewrite H6. rewrite H4. unfold varg_proj.
     destruct v1; 
@@ -1819,7 +1070,7 @@ Proof.
     inv H5; inv H13; inv H4; inv H16; inv H6; inv H8.
     inv H7; inv H5; inv H3; simpl in H4.
       (*S exists*)
-      inv sfrel; unfold S_proj; unfold param_val. rewrite H8; rewrite H7.
+      inv sfrel; unfold bit_proj; unfold param_val. rewrite H8; rewrite H7.
       unfold varg_proj.
       destruct v2; simpl; try auto;
       unfold sem_cmp in H1; simpl in H1; inv H1.
@@ -1834,7 +1085,7 @@ Proof.
         inv H19; inv H14; inv H20; inv H0; inv H6; inv H10; inv H5. 
         inv H1.
           (*d exists*)
-          inv dfrel; unfold d_proj; unfold param_val.
+          inv dfrel; unfold reg_proj; unfold param_val.
           rewrite H10. rewrite H6.
           unfold varg_proj.
           destruct v0;
@@ -1851,7 +1102,7 @@ Proof.
       inv H1;
         (*d exists*)
         unfold sem_binary_operation in H11; unfold sem_cmp in H11; simpl in H11.
-        inv dfrel; unfold d_proj; unfold param_val.
+        inv dfrel; unfold reg_proj; unfold param_val.
         rewrite H10; rewrite H6.
         unfold varg_proj.
         destruct v0; inv H11. 
@@ -1864,7 +1115,7 @@ Proof.
     (*false*)
     inv H10; inv H0. inv H5. inv H7. inv H2.
       (*S exist*)
-      inv sfrel; unfold S_proj; unfold param_val. 
+      inv sfrel; unfold bit_proj; unfold param_val. 
       rewrite H7; rewrite H6.
       unfold varg_proj.
       destruct v2; simpl; try auto;
@@ -1893,7 +1144,7 @@ Proof.
     inv H5; inv H13; inv H4; inv H16; inv H6; inv H8.
     inv H7; inv H5; inv H3; simpl in H4.
       (*S exists*)
-      inv sfrel; unfold S_proj; unfold param_val; 
+      inv sfrel; unfold bit_proj; unfold param_val; 
       rewrite H8; rewrite H7;
       unfold varg_proj.
       destruct v2; simpl; try auto;
@@ -1913,7 +1164,7 @@ Proof.
           (*d exists*)
           unfold sem_binary_operation in H11; simpl in H11;
           unfold sem_cmp in H11; simpl in H11; inv H11.
-          inv dfrel; unfold d_proj; unfold param_val; unfold varg_proj.
+          inv dfrel; unfold reg_proj; unfold param_val; unfold varg_proj.
           rewrite H10; rewrite H6.
           destruct v0; inv H0.
             (*d is int*)
@@ -1928,7 +1179,7 @@ Proof.
     inv H10. inv H0. inv H14. inv H7. inv H5.
     inv H2.
       (*S exists*)
-      inv sfrel; unfold S_proj; unfold param_val; unfold varg_proj.
+      inv sfrel; unfold bit_proj; unfold param_val; unfold varg_proj.
       rewrite H7; rewrite H6.
       destruct v2; inv H1.
       (*S is int*)
@@ -1940,39 +1191,183 @@ Qed.
 
 (* Lemmas on if CurrentModeHasSPSR *)
 Definition hasSPSR :=
-  Ecall (Evalof (Evar CurrentModeHasSPSR T10) T10)
-  (Econs (Evalof (Evar proc T3) T3) Enil) T10.
+  Ecall (Evalof (Evar CurrentModeHasSPSR T12) T12)
+  (Econs (Evalof (Evar proc T3) T3) Enil) T4.
 
 Axiom if_hasSPSR_ok :
   forall e m t m' v,
     eval_expression (Genv.globalenv prog_adc) e m hasSPSR t m' v ->
     m = m'/\eval_expression (Genv.globalenv prog_adc) e m hasSPSR t m' v.
 
-Lemma hasSPSR_true :
-  forall e m t m' v s em,
+Lemma hasSPSR_true' :
+  forall m0 m0' e m vargs t m' v l b s,
+    alloc_variables empty_env m0 
+      (fun_internal_ADC.(fn_params) ++ fun_internal_ADC.(fn_vars)) e m0' ->
+    bind_parameters e m0' fun_internal_ADC.(fn_params) vargs m ->
     eval_expression (Genv.globalenv prog_adc) e m hasSPSR t m' v ->
-    Csem.is_true v T10 ->
+    proc_state_related (of_mem proc m') e (Ok tt (mk_semstate l b s)) ->
+    Csem.is_true v T4 ->
+    word_of_proc_mode (mode_proj m' e) < 5.
+Proof.
+  intros until s. intros av bp hs psrel tr.
+
+  inv hs. inv H. inv H0. 
+  (* m = m3 *)
+  inv H4. inv H3. inv H5. inv H3. inv H4. inv H13.
+  (* ? *)
+  inv H6.
+  (* expand local env e *)
+  inv av. inv H14. inv H17. inv H18. inv H19. inv H20. inv H21. inv H22.
+  pose (e:=
+    PTree.set old_Rn (b7, Tint I32 Unsigned)
+      (PTree.set shifter_operand (b6, Tint I32 Unsigned)
+        (PTree.set n (b5, Tint I8 Unsigned)
+          (PTree.set d (b4, Tint I8 Unsigned)
+            (PTree.set cond (b3, Tint I32 Signed)
+              (PTree.set S (b2, Tint I8 Unsigned)
+                (PTree.set proc (b1, Tpointer typ_SLv6_Processor)
+                  empty_env))))))).
+  fold e in psrel, bp, H7. fold e. 
+  (* CurrentModeHasSPSR is in global env *)
+  inv H1; [simpl in H6; discriminate H6| clear H3].
+  (* search CurrentModeHasSPSR in global env *)
+  (* vf=Vptr (-6) w0 *)
+  inv H5. unfold load_value_of_type in H4; simpl in H4. 
+  injection H4; intro; clear H4. rewrite <- H in *; clear vf H.
+  (* fd = fun_Internal_CurrentModeHasSPSR *)
+  inversion H11;  destruct eq_dec; 
+    [clear e0 H11 H2 H12 H8; inv H0|discriminate H0].
+
+  (* pass parameter proc to internal function CurrentModeHasSPSR *)
+  inv H7. inv H5. 
+  (* v0 is value of proc *)
+  inv H1; clear H4.
+  inv H3;
+  [unfold e in H5;simpl in H5;injection H5;intro;rewrite<-H in *;clear b0 H H5
+  |unfold e in H1;simpl in H1;discriminate H1].
+
+
+  (* open CrrentModeHasSPSR *)
+  inv H16. inv H4. 
+  (* return value is v (cast from v1) *)
+  simpl in H5; destruct H5.
+  (* m9 = m10 *)
+  inv H11. inv H5. inv H27. inv H26. inv H16. inv H25. inv H24. inv H16. inv H21.
+  (* arguments v2,v3 of binary operation lt*)
+  inv H7. simpl in H23.
+  (* v3 = 5 *)
+  inv H22.
+  (* v2 = v0 *)
+  inv H21; clear H11.
+  (* typ_struct_SLv6_StatusRegister is a structure *)
+  inv H9;[idtac|simpl in H24;unfold T7 in H24;discriminate H24].
+  inv H24.
+  (* offset of mode is 16 *)
+  assert (field_offset mode typ_struct_SLv6_StatusRegister = OK 16).  
+  unfold field_offset. simpl. 
+  Ltac unfold_identeq :=
+    destruct AST.ident_eq;
+      [try (unfold align;simpl;discriminate||destruct AST.ident_eq)
+        |try unfold_identeq].
+  unfold_identeq. unfold align. simpl. reflexivity. admit.
+  rewrite H5 in H25; clear H5. 
+  injection H25;intro;rewrite<-H5 in H16;clear H5 H25 delta.
+  (* typ_struct_SLv6_Processor is a structure *)    
+  inv H12; [idtac|simpl in H24;unfold T6 in H24;discriminate H24].
+  inv H24.
+  (* offset of cpsr  is 2 *)
+  assert (field_offset cpsr typ_struct_SLv6_Processor = OK 2). admit.
+  rewrite H5 in H25; clear H5. 
+  injection H25; intro; rewrite<-H5 in H16; clear delta H5 H25.
+  (* expand e0 *)
+  inv H1. inv H26.   
+  (* proc is in e0 *)
+  inv H11. inv H12. inv H7;[idtac|simpl in H11; discriminate H11]. clear H9.
+  (* b9 = b8 *)
+  simpl in H22; injection H22;intro;rewrite<-H1 in *; clear b9 H22 H1.
+  (* load v0 from b9 *)
+  inv H3.
+  inv H28; simpl in H26;injection H26;intro;rewrite<-H1 in *;clear b9 H1 H26.
+  unfold store_value_of_type in H27;simpl in H27.
+  generalize H27; intro bp'.
+  apply Mem.load_store_same in H27;
+    [idtac|simpl;destruct v0;simpl;try(exact I||inv H2)].
+  unfold load_value_of_type in *; simpl in H6, H16, H21.
+  rewrite H27 in H21. 
+  injection H21; intro. destruct v0; try discriminate H1.
+  injection H1; intros; rewrite<-H3,H5 in *;clear H1 H3 H5.
+  simpl in H27.
+  (* v' = Vptr b0 i*)
+  inv H2.
+  unfold sem_cmp in H23; simpl in H23.
+  destruct v2; try discriminate H23.
+  injection H23; intro; clear H23. rewrite <- H1 in *; clear H1.
+
+  (* unfold goal *)
+  unfold mode_proj. unfold find_mode. unfold find_cpsr. unfold find_field.
+  unfold proc_loc. 
+  unfold e. Set Printing Depth 50. simpl. unfold load_value_of_type; simpl.
+  (* b1 not change between m3 m8 *)
+  generalize H6;intro.
+  apply (Mem.load_alloc_other m3 0 (sizeof (Tpointer typ_SLv6_Processor))
+    m8 b8 H25) in H6. 
+  (* b1 not changed between m8 m10 *)
+  (*apply load_store*)
+Admitted.
+
+Lemma hasSPSR_true :
+  forall m0 m0' m0'' e m vargs t m' v l b s em,
+    alloc_variables empty_env m0 
+      (fun_internal_ADC.(fn_params) ++ fun_internal_ADC.(fn_vars)) e m0' ->
+    bind_parameters e m0' fun_internal_ADC.(fn_params) vargs m0'' ->
+    eval_expression (Genv.globalenv prog_adc) e m hasSPSR t m' v ->
+    proc_state_related (of_mem proc m') e (Ok tt (mk_semstate l b s)) ->
+    Csem.is_true v T4 ->
     Arm6_State.mode s = exn  em.
 Proof.
-  intros until em. intros hasspsr has_true.
-  inv has_true.
-Qed.
+  intros until em. intros av bp hs psrel tr.
+  inv hs. inv H. inv H0. inv H4. inv H3. inv H5. inv H3. inv H4. inv H13.
+  inv H6.
+  inv av. inv H14. inv H17. inv H18. inv H19. inv H20. inv H21. inv H22.
+  pose (e:=
+    PTree.set old_Rn (b7, Tint I32 Unsigned)
+            (PTree.set shifter_operand (b6, Tint I32 Unsigned)
+               (PTree.set n (b5, Tint I8 Unsigned)
+                  (PTree.set d (b4, Tint I8 Unsigned)
+                     (PTree.set cond (b3, Tint I32 Signed)
+                        (PTree.set S (b2, Tint I8 Unsigned)
+                           (PTree.set proc (b1, Tpointer typ_SLv6_Processor)
+                              empty_env))))))).
+  fold e in psrel, bp, H7. inv H1. simpl in H6; discriminate H6. simpl in H3.
+  inv H5. inv H4. inv H11. 
+  destruct eq_dec; [clear e0|discriminate H0].
+  clear H2 H12. inv H0. inv H7. inversion H8; clear H8. 
+  rewrite <- H0 in *; clear H0. rewrite <- H4 in *; clear H4. clear H5.
+  inv H6.
+  
+  inv H1. clear H5. 
+  inv H4; [idtac|unfold e in H1; simpl in H1; discriminate H1].
+  unfold e in H6; simpl in H6; inversion H6. rewrite <- H0 in *; clear b0 H0 H6.
+  unfold load_value_of_type in H7; simpl in H7.
+
+  (* open CrrentModeHasSPSR *)
+  inv H16. inv H5. simpl in H6. destruct H6.
+
+Admitted.
 
 Lemma hasSPSR_false :
   forall e m t m' v s,
     eval_expression (Genv.globalenv prog_adc) e m hasSPSR t m' v ->
-    Csem.is_false v T10 ->
+    Csem.is_false v T4 ->
     Arm6_State.mode s = usr.
 Proof.
-  intros until s. intros hasspsr has_false.
-  inv has_false.
-Qed.
+Admitted.
 
 (*Lemma on proc_state_relates holds after copy_StatusRegister*)
 Definition get_spsr :=
-  Ecall (Evalof (Evar spsr T6) T6)
+  Ecall (Evalof (Evar spsr T14) T14)
   (Econs (Evalof (Evar proc T3) T3)
-    Enil) T6.
+    Enil) T8.
 
 Axiom get_spsr_ok:
   forall e m t m' r,
@@ -1981,13 +1376,16 @@ Axiom get_spsr_ok:
 
 Definition cp_SR :=
   Ecall
-  (Evalof (Evar copy_StatusRegister T11) T11)
+  (Evalof (Evar copy_StatusRegister T13) T13)
   (Econs
     (Eaddrof
       (Efield
         (Ederef (Evalof (Evar proc T3) T3) T6)
-        cpsr T6) T6)
-    (Econs get_spsr Enil)) T9.
+        cpsr T7) T8)
+    (Econs
+      (Ecall (Evalof (Evar spsr T14) T14)
+        (Econs (Evalof (Evar proc T3) T3)
+          Enil) T8) Enil)) T11.
 
 Lemma same_cp_SR :
   forall e m l b s t m' v em,
@@ -2018,7 +1416,7 @@ Qed.
    For the moment, we consider it as a function call with an 
    empty body *)
 Definition unpred :=
-  Ecall (Evalof (Evar adc_compcert_fixed.unpredicatable T9) T9) Enil T9.
+  (Ecall (Evalof (Evar unpredicatable T15) T15) Enil T11).
 
 Lemma same_unpred :
   forall e m s t m' v,
@@ -2034,16 +1432,22 @@ Proof.
 Qed.
 
 (* Lemma on proc_state_relates holds after NZCV flag setting*)
-(*Definition nflag_assgnt:=
+Definition nflag_assgnt:=
   Eassign
   (Efield
     (Efield
-      (Ederef (Evalof (Evar proc T3) T3)
-        (Tpointer T3)) cpsr T6) N_flag T4)
-  (Ecall (Evalof (Evar get_bit T12) T12)
-    (Econs (reg_id d)
-      (Econs (Eval (Vint (repr 31)) T7)
+      (Ederef (Evalof (Evar proc T3) T3) T6)
+      cpsr T7) N_flag T4)
+  (Ecall (Evalof (Evar get_bit T16) T16)
+    (Econs
+      (Ecall (Evalof (Evar reg T2) T2)
+        (Econs (Evalof (Evar proc T3) T3)
+          (Econs 
+            (Evalof (Evar d T4) T4) Enil))
+        T1)
+      (Econs (Eval (Vint (repr 31)) T9)
         Enil)) T4) T4.
+
 Lemma same_nflag_assgnt :
   forall e m l b s d t m' v,
   proc_state_related (of_mem proc m) e (Ok tt (mk_semstate l b s)) ->
@@ -2058,21 +1462,15 @@ Lemma same_nflag_assgnt :
          )
     ).
 Proof.
-  intros until v. intros psrel dfrel nf. intros.
-  inv nf. inv H. simpl in *. inv H4. inv H14. inv H13. inv H4.
-  inv H8. inv H5. inv H3. inv H13. inv H4. 
-  eapply get_reg_ok in H5. subst.
-  inv H19. inv H4. 
-Admitted.*)
+Admitted.
 
 Definition zflag_assgnt :=
   Eassign
   (Efield
     (Efield
       (Ederef 
-        (Evalof (Evar proc T3) T3)
-        (Tpointer T3)) cpsr T6) Z_flag
-    T4)
+        (Evalof (Evar proc T3) T3) T6)
+      cpsr T7) Z_flag T4)
   (Econdition
     (Ebinop Oeq
       (Ecall (Evalof (Evar reg T2) T2)
@@ -2081,9 +1479,9 @@ Definition zflag_assgnt :=
           (Econs
             (Evalof (Evar d T4) T4)
             Enil)) T1)
-      (Eval (Vint (repr 0)) T7) T7)
-    (Eval (Vint (repr 1)) T7)
-    (Eval (Vint (repr 0)) T7) T7) T4.
+      (Eval (Vint (repr 0)) T9) T9)
+    (Eval (Vint (repr 1)) T9)
+    (Eval (Vint (repr 0)) T9) T9) T4.
 
 Lemma same_zflag_assgnt :
   forall e m l b s d t m' v,
@@ -2096,9 +1494,6 @@ Lemma same_zflag_assgnt :
          then repr 1
          else repr 0)))).
 Proof.
-  intros until v. intros psrel dfrel zf.
-  inv zf. inv H. simpl in H15.
-  inv H15.
 Admitted.
 
 Definition cflag_assgnt:=
@@ -2107,11 +1502,10 @@ Definition cflag_assgnt:=
     (Efield
       (Ederef
         (Evalof (Evar proc T3) T3)
-        (Tpointer T3)) cpsr T6)
-    C_flag T4)
+        T6) cpsr T7) C_flag T4)
   (Ecall
     (Evalof 
-      (Evar CarryFrom_add3 T9) T9)
+      (Evar CarryFrom_add3 T17) T17)
     (Econs
       (Evalof (Evar old_Rn T1) T1)
       (Econs
@@ -2124,9 +1518,8 @@ Definition cflag_assgnt:=
               (Efield
                 (Ederef
                   (Evalof (Evar proc T3) T3)
-                  (Tpointer T3)) cpsr T6)
-              C_flag T4) T4) Enil))) T4)
-  T4.
+                  T6) cpsr T7) C_flag T4) T4)
+          Enil))) T4) T4.
 
 Lemma same_cflag_assgnt:
   forall m e l b s0 s n so t m' v,
@@ -2139,9 +1532,6 @@ Lemma same_cflag_assgnt:
         (Arm6_Functions.CarryFrom_add3 (Arm6_State.reg_content s0 n) so
           (Arm6_State.cpsr (st (mk_semstate l b s))) [Cbit])))).
 Proof.
-  intros until v. intros psrel nfrel sofrel cf.
-  inv cf. inv H. simpl in H15.
-  inv H15.
 Admitted.
 
 Definition vflag_assgnt:=
@@ -2150,15 +1540,13 @@ Definition vflag_assgnt:=
     (Efield
       (Ederef
         (Evalof (Evar proc T3) T3)
-        (Tpointer T3)) cpsr T6)
-    V_flag T4)
+        T6) cpsr T7) V_flag T4)
   (Ecall
     (Evalof
-      (Evar OverflowFrom_add3 T9) T9)
+      (Evar OverflowFrom_add3 T18)
+      T18)
     (Econs
-      (Evalof
-        (Evalof (Evar old_Rn T1) T1)
-        T1)
+      (Evalof (Evar old_Rn T1) T1)
       (Econs
         (Evalof
           (Evar shifter_operand T1)
@@ -2169,9 +1557,9 @@ Definition vflag_assgnt:=
               (Efield
                 (Ederef
                   (Evalof (Evar proc T3) T3)
-                  (Tpointer T3)) cpsr T6)
-              C_flag T4) T4) Enil))) T4)
-  T4.
+                  T6) cpsr T7) C_flag T4) T4)
+          Enil))) T4) T4.
+
 Lemma same_vflag_assgnt:
   forall m e l b s0 s n so t m' v,
     proc_state_related (of_mem proc m) e (Ok tt (mk_semstate l b s)) ->
@@ -2183,9 +1571,6 @@ Lemma same_vflag_assgnt:
         (Arm6_Functions.OverflowFrom_add3 (Arm6_State.reg_content s0 n) so
            (Arm6_State.cpsr (st (mk_semstate l b s))) [Cbit])))).
 Proof.
-  intros until v. intros psrel nfrel sofrel vf.
-  inv vf. inv H. simpl in H15.
-  inv H15.
 Admitted.
 
 
@@ -2195,12 +1580,6 @@ Lemma cp_SR_params_not_changed:
     eval_expression (Genv.globalenv prog_adc) e m cp_SR Events.E0 m' v ->
     param_val i m e = param_val i m' e.
 Proof.
-  intros until i. intros ex.
-  inv ex. inv H. inv H5. inv H9.
-  inv H6. inv H5. inv H6. inv H17. inv H5. inv H6.
-  inv H15. inv H14.
-  inv H5. inv H3. inv H15. inv H6. inv H21.
-  inv H5. inv H6. simpl in *.
 Admitted.
 
 Lemma reg_S_not_changed :
@@ -2209,10 +1588,6 @@ Lemma reg_S_not_changed :
     vargs t m' v ->
     param_val S m e = param_val S m' e.
 Proof.
-  intros until v. intro evfun.
-  inv evfun.
-
-
 Admitted.
 
 
@@ -2439,6 +1814,7 @@ Lemma rn_ass_params_not_changed:
     eval_expression (Genv.globalenv prog_adc) e m oldrn_assgnt Events.E0 m' v ->
     param_val i m e = param_val i m' e.
 Proof.
+Admitted.
 
 Lemma set_reg_params_not_changed:
   forall m e v m' i, 
@@ -2488,8 +1864,8 @@ Proof.
 Qed.
 
 Theorem related_aft_ADC: forall e m0 m1 m2 mfin vargs s out sbit cond d n so,
-  alloc_variables empty_env m0 (ADC_body.(fn_params) ++ ADC_body.(fn_vars)) e m1 ->
-  bind_parameters e m1 ADC_body.(fn_params) vargs m2 ->
+  alloc_variables empty_env m0 (fun_internal_ADC.(fn_params) ++ fun_internal_ADC.(fn_vars)) e m1 ->
+  bind_parameters e m1 fun_internal_ADC.(fn_params) vargs m2 ->
 (* TODO: valid_access needs to be more precise *)
   (forall m ch b ofs, Mem.valid_access m ch b ofs Readable) ->
   proc_state_related (of_mem proc m2) e (Ok tt (mk_semstate nil true s)) ->
@@ -2513,7 +1889,7 @@ Theorem related_aft_ADC: forall e m0 m1 m2 mfin vargs s out sbit cond d n so,
    statement execution [Out_break], [Out_continue], [Out_normal] and [Out_return].
    The final memory state is the memory which contains the final values of parameters.
    The final [proc] is in this memory state which we want to relate.*)
-  exec_stmt (Genv.globalenv prog_adc) e m2 ADC_body.(fn_body) Events.E0 mfin out ->
+  exec_stmt (Genv.globalenv prog_adc) e m2 fun_internal_ADC.(fn_body) Events.E0 mfin out ->
   proc_state_related (of_mem proc mfin) e (S.ADC_step sbit cond d n so (mk_semstate nil true s)). 
 Proof.
   
@@ -2527,26 +1903,26 @@ Proof.
   rename H2 into rn_assgnt.
   apply (oldrn_assgnt_ok e m2 nil true s Events.E0 m3 v) in psrel; 
     [idtac|exact rn_assgnt];
-  unfold sbit_func_related in sfrel; unfold S_proj in sfrel;
+  unfold sbit_func_related in sfrel; unfold bit_proj in sfrel;
   rewrite (rn_ass_params_not_changed m2 e v m3 S) in sfrel;
     [idtac | exact rn_assgnt];
-  fold (S_proj m3 e) in sfrel; fold (sbit_func_related m3 e sbit) in sfrel.
+  fold (bit_proj m3 e S) in sfrel; fold (sbit_func_related m3 e sbit) in sfrel.
   unfold cond_func_related in cfrel; unfold cond_proj in cfrel;
   rewrite (rn_ass_params_not_changed m2 e v m3 adc_compcert_fixed.cond) in cfrel;
     [idtac | exact rn_assgnt];
   fold (cond_proj m3 e) in cfrel; fold (cond_func_related m3 e cond) in cfrel.
-  unfold d_func_related in dfrel; unfold d_proj in dfrel;
+  unfold d_func_related in dfrel; unfold reg_proj in dfrel;
   rewrite (rn_ass_params_not_changed m2 e v m3 adc_compcert_fixed.d) in dfrel;
     [idtac | exact rn_assgnt];
-  fold (d_proj m3 e) in dfrel; fold (d_func_related m3 e d) in dfrel.
-  unfold n_func_related in nfrel; unfold n_proj in nfrel;
+  fold (reg_proj m3 e adc_compcert_fixed.d) in dfrel; fold (d_func_related m3 e d) in dfrel.
+  unfold n_func_related in nfrel; unfold reg_proj in nfrel;
   rewrite (rn_ass_params_not_changed m2 e v m3 adc_compcert_fixed.n) in nfrel;
     [idtac | exact rn_assgnt]; 
-  fold (n_proj m3 e) in nfrel; fold (n_func_related m3 e n) in nfrel.
-  unfold so_func_related in sofrel; unfold so_proj in sofrel;
+  fold (reg_proj m3 e adc_compcert_fixed.n) in nfrel; fold (n_func_related m3 e n) in nfrel.
+  unfold so_func_related in sofrel; unfold bits_proj in sofrel;
   rewrite (rn_ass_params_not_changed m2 e v m3 shifter_operand) in sofrel;
     [clear rn_assgnt | exact rn_assgnt];
-  fold (so_proj m3 e) in sofrel; fold (so_func_related m3 e so) in sofrel (* m2=m3 *).
+  fold (bits_proj m3 e shifter_operand) in sofrel; fold (so_func_related m3 e so) in sofrel (* m2=m3 *).
   inv main_p;
   rename H5 into condpass, H8 into cp_b, H9 into main_p, H4 into evs;
       simpl in cp_b;
@@ -2556,37 +1932,39 @@ Proof.
       rewrite H in * |- *; clear H condpass0;
       rename H0 into condpass.
     (* ConditionPassed(&proc->cpsr, cond) evaluates to true *)
-    apply (condpass_true e m4 Events.E0 m4 v1 cond s) in cp_b;
-      [idtac | inv cp_b].
+    apply (condpass_true m0 m1 e m4 Events.E0 m4 v1 cond s) in cp_b;
+    [idtac| exact al| exact condpass].
+      (*[idtac |exact al | inv cp_b].*)
 
     inv main_p; [idtac | nod];
     rename H4 into setreg, H7 into main_p, H3 into evs;
     apply Events.Eapp_E0_inv in evs; destruct evs; subst.
+
     inv setreg;
     rename H2 into setreg;
     apply (same_setregpc e m4 nil true s s Events.E0 m5 v0 d n so) 
       with nil (Util.zne d 15) in psrel;
-      [idtac | apply setreg].
-    unfold sbit_func_related in sfrel; unfold S_proj in sfrel;   
+      [idtac | fold set_regpc in setreg; apply setreg].
+    unfold sbit_func_related in sfrel; unfold bit_proj in sfrel;   
     rewrite (set_reg_params_not_changed m4 e v0 m5 S) in sfrel;
       [idtac | exact setreg];
-    fold (S_proj m5 e) in sfrel; fold (sbit_func_related m5 e sbit) in sfrel.
+    fold (bit_proj m5 e S) in sfrel; fold (sbit_func_related m5 e sbit) in sfrel.
     unfold cond_func_related in cfrel; unfold cond_proj in cfrel;
     rewrite (set_reg_params_not_changed m4 e v0 m5 adc_compcert_fixed.cond) in cfrel;
       [idtac | exact setreg];
     fold (cond_proj m5 e) in cfrel; fold (cond_func_related m5 e cond) in cfrel.
-    unfold d_func_related in dfrel; unfold d_proj in dfrel;
+    unfold d_func_related in dfrel; unfold reg_proj in dfrel;
     rewrite (set_reg_params_not_changed m4 e v0 m5 adc_compcert_fixed.d) in dfrel;
       [idtac | exact setreg];
-    fold (d_proj m5 e) in dfrel; fold (d_func_related m5 e d) in dfrel.
-    unfold n_func_related in nfrel; unfold n_proj in nfrel;
+    fold (reg_proj m5 e adc_compcert_fixed.d) in dfrel; fold (d_func_related m5 e d) in dfrel.
+    unfold n_func_related in nfrel; unfold reg_proj in nfrel;
     rewrite (set_reg_params_not_changed m4 e v0 m5 adc_compcert_fixed.n) in nfrel;
       [idtac | exact setreg]; 
-    fold (n_proj m5 e) in nfrel; fold (n_func_related m5 e n) in nfrel.
-    unfold so_func_related in sofrel; unfold so_proj in sofrel;
+    fold (reg_proj m5 e adc_compcert_fixed.n) in nfrel; fold (n_func_related m5 e n) in nfrel.
+    unfold so_func_related in sofrel; unfold bits_proj in sofrel;
     rewrite (set_reg_params_not_changed m4 e v0 m5 shifter_operand) in sofrel;
       [clear setreg | exact setreg];
-    fold (so_proj m5 e) in sofrel; fold (so_func_related m5 e so) in sofrel (*m4 -> m5*).
+    fold (bits_proj m5 e shifter_operand) in sofrel; fold (so_func_related m5 e so) in sofrel (*m4 -> m5*).
     inv main_p;
     rename H5 into sd, H8 into sd_b, H9 into main_p, H4 into evs;
         simpl in sd_b;
@@ -2609,38 +1987,39 @@ Proof.
         (* CurrentModeHasSPSR(proc) evaluates to true *)
         inv main_p;
         rename H2 into cp_sr.
+        generalize psrel; intro psrelm7.
         apply (same_cp_SR e m7 nil (Util.zne d 15) 
           (Arm6_State.set_reg s d
           (add (add (Arm6_State.reg_content s n) so)
             (Arm6_State.cpsr s) [Cbit])) Events.E0 mfin v4 und) 
         with nil (Util.zne d 15) in psrel;
           [idtac | exact cp_sr ].
-        unfold sbit_func_related in sfrel; unfold S_proj in sfrel;   
+        unfold sbit_func_related in sfrel; unfold bit_proj in sfrel;   
         rewrite (cp_SR_params_not_changed m7 e v4 mfin S) in sfrel;
           [idtac | exact cp_sr];
-        fold (S_proj mfin e) in sfrel; fold (sbit_func_related mfin e sbit) in sfrel.
+        fold (bit_proj mfin e S) in sfrel; fold (sbit_func_related mfin e sbit) in sfrel.
         unfold cond_func_related in cfrel; unfold cond_proj in cfrel;
-        rewrite (cp_SR_params_not_changed m7 e v4 mfin adc_compcert.cond) in cfrel;
+        rewrite (cp_SR_params_not_changed m7 e v4 mfin adc_compcert_fixed.cond) in cfrel;
           [idtac | exact cp_sr];
         fold (cond_proj mfin e) in cfrel; fold (cond_func_related mfin e cond) in cfrel.
-        unfold d_func_related in dfrel; unfold d_proj in dfrel;
-        rewrite (cp_SR_params_not_changed m7 e v4 mfin adc_compcert.d) in dfrel;
+        unfold d_func_related in dfrel; unfold reg_proj in dfrel;
+        rewrite (cp_SR_params_not_changed m7 e v4 mfin adc_compcert_fixed.d) in dfrel;
           [idtac | exact cp_sr];
-        fold (d_proj mfin e) in dfrel; fold (d_func_related mfin e d) in dfrel.
-        unfold n_func_related in nfrel; unfold n_proj in nfrel;
-        rewrite (cp_SR_params_not_changed m7 e v4 mfin adc_compcert.n) in nfrel;
+        fold (reg_proj mfin e adc_compcert_fixed.d) in dfrel; fold (d_func_related mfin e d) in dfrel.
+        unfold n_func_related in nfrel; unfold reg_proj in nfrel;
+        rewrite (cp_SR_params_not_changed m7 e v4 mfin adc_compcert_fixed.n) in nfrel;
           [idtac | exact cp_sr]; 
-        fold (n_proj mfin e) in nfrel; fold (n_func_related mfin e n) in nfrel.
-        unfold so_func_related in sofrel; unfold so_proj in sofrel;
+        fold (reg_proj mfin e adc_compcert_fixed.n) in nfrel; fold (n_func_related mfin e n) in nfrel.
+        unfold so_func_related in sofrel; unfold bits_proj in sofrel;
         rewrite (cp_SR_params_not_changed m7 e v4 mfin shifter_operand) in sofrel;
           [clear cp_sr | exact cp_sr];
-        fold (so_proj mfin e) in sofrel; fold (so_func_related mfin e so) in sofrel (*m7->mfin*).
-        apply (hasSPSR_true e m6 Events.E0 m7 v3
+        fold (bits_proj mfin e shifter_operand) in sofrel; fold (so_func_related mfin e so) in sofrel (*m7->mfin*).
+        apply (hasSPSR_true m0 m1 m2 e m7 vargs Events.E0 m7 v3 nil (Util.zne d 15)
           (Arm6_State.set_reg s d
             (add (add (Arm6_State.reg_content s n) so)
               (Arm6_State.cpsr s) [Cbit]))
           und) in spsr_b;
-          [idtac |inv spsr_b].
+          [idtac |exact al|exact bi|exact hasspsr|exact psrelm7].
         unfold S.ADC_step; unfold _get_st; unfold bind_s;
           unfold bind; simpl.
         rewrite cp_b; rewrite sd; simpl.
@@ -2649,7 +2028,7 @@ Proof.
         unfold _Arm_State.set_reg.
         rewrite spsr_b; simpl; unfold _Arm_State.set_reg; unfold _Arm_State.set_cpsr.
         unfold _set_bo; unfold ok_semstate. unfold loc. unfold st. rewrite same_bool.
-        apply psrel.
+        exact psrel. (*exact hasspsr. exact hasspsr.*)
         (* CurrentModeHasSPSR(proc) evaluates to false *)
         inv main_p; rename H2 into unp.
         apply (same_unpred e m7 
@@ -2658,30 +2037,30 @@ Proof.
                     (Arm6_State.cpsr s) [Cbit])))
                 Events.E0 mfin v4) in psrel;
         [idtac | exact unp].
-        unfold sbit_func_related in sfrel; unfold S_proj in sfrel;   
+        unfold sbit_func_related in sfrel; unfold bit_proj in sfrel;   
         rewrite (unpred_params_not_changed m7 e v4 mfin S) in sfrel;
           [idtac | exact unp];
-        fold (S_proj mfin e) in sfrel; fold (sbit_func_related mfin e sbit) in sfrel.
+        fold (bit_proj mfin e S) in sfrel; fold (sbit_func_related mfin e sbit) in sfrel.
         unfold cond_func_related in cfrel; unfold cond_proj in cfrel;
         rewrite (unpred_params_not_changed m7 e v4 mfin adc_compcert_fixed.cond) in cfrel;
           [idtac | exact unp];
         fold (cond_proj mfin e) in cfrel; fold (cond_func_related mfin e cond) in cfrel.
-        unfold d_func_related in dfrel; unfold d_proj in dfrel;
+        unfold d_func_related in dfrel; unfold reg_proj in dfrel;
         rewrite (unpred_params_not_changed m7 e v4 mfin adc_compcert_fixed.d) in dfrel;
           [idtac | exact unp];
-        fold (d_proj mfin e) in dfrel; fold (d_func_related mfin e d) in dfrel.
-        unfold n_func_related in nfrel; unfold n_proj in nfrel;
+        fold (reg_proj mfin e adc_compcert_fixed.d) in dfrel; fold (d_func_related mfin e d) in dfrel.
+        unfold n_func_related in nfrel; unfold reg_proj in nfrel;
         rewrite (unpred_params_not_changed m7 e v4 mfin adc_compcert_fixed.n) in nfrel;
           [idtac | exact unp]; 
-        fold (n_proj mfin e) in nfrel; fold (n_func_related mfin e n) in nfrel.
-        unfold so_func_related in sofrel; unfold so_proj in sofrel;
+        fold (reg_proj mfin e adc_compcert_fixed.n) in nfrel; fold (n_func_related mfin e n) in nfrel.
+        unfold so_func_related in sofrel; unfold bits_proj in sofrel;
         rewrite (unpred_params_not_changed m7 e v4 mfin shifter_operand) in sofrel;
           [clear unp | exact unp];
-        fold (so_proj mfin e) in sofrel; fold (so_func_related mfin e so) in sofrel.
+        fold (bits_proj mfin e shifter_operand) in sofrel; fold (so_func_related mfin e so) in sofrel.
         unfold S.ADC_step; unfold _get_st; unfold bind_s;
         unfold bind; simpl.
         rewrite cp_b; rewrite sd; simpl.
-        apply (hasSPSR_false e m6 Events.E0 m7 v3
+        apply (hasSPSR_false e m7 Events.E0 m7 v3
           (Arm6_State.set_reg s d
             (add (add (Arm6_State.reg_content s n) so)
               (Arm6_State.cpsr s) [Cbit]))
@@ -2691,7 +2070,7 @@ Proof.
         unfold _get_bo. unfold bind_s. unfold next. unfold bind.
         simpl; unfold _Arm_State.set_reg.
         rewrite spsr_b; simpl.
-        exact psrel.
+        exact psrel. exact hasspsr. 
       (* ((S == 1) && (d == 15)) evaluates to false *)
       apply (S_set_and_is_pc_false e m6 Events.E0 m6 v2 sbit d) in sd_b;
         [idtac|exact sfrel|exact dfrel|exact sd].
@@ -2721,26 +2100,26 @@ Proof.
           in psrel;
           [idtac | exact dfrel | exact nf].
 
-        unfold sbit_func_related in sfrel; unfold S_proj in sfrel;   
+        unfold sbit_func_related in sfrel; unfold bit_proj in sfrel;   
         rewrite (nf_params_not_changed m7 e v4 m8 S) in sfrel;
           [idtac | exact nf];
-        fold (S_proj m8 e) in sfrel; fold (sbit_func_related m8 e sbit) in sfrel.
+        fold (bit_proj m8 e S) in sfrel; fold (sbit_func_related m8 e sbit) in sfrel.
         unfold cond_func_related in cfrel; unfold cond_proj in cfrel;
         rewrite (nf_params_not_changed m7 e v4 m8 adc_compcert_fixed.cond) in cfrel;
           [idtac | exact nf];
         fold (cond_proj m8 e) in cfrel; fold (cond_func_related m8 e cond) in cfrel.
-        unfold d_func_related in dfrel; unfold d_proj in dfrel;
+        unfold d_func_related in dfrel; unfold reg_proj in dfrel;
         rewrite (nf_params_not_changed m7 e v4 m8 adc_compcert_fixed.d) in dfrel;
           [idtac | exact nf];
-        fold (d_proj m8 e) in dfrel; fold (d_func_related m8 e d) in dfrel.
-        unfold n_func_related in nfrel; unfold n_proj in nfrel;
+        fold (reg_proj m8 e adc_compcert_fixed.d) in dfrel; fold (d_func_related m8 e d) in dfrel.
+        unfold n_func_related in nfrel; unfold reg_proj in nfrel;
         rewrite (nf_params_not_changed m7 e v4 m8 adc_compcert_fixed.n) in nfrel;
           [idtac | exact nf]; 
-        fold (n_proj m8 e) in nfrel; fold (n_func_related m8 e n) in nfrel.
-        unfold so_func_related in sofrel; unfold so_proj in sofrel;
+        fold (reg_proj m8 e adc_compcert_fixed.n) in nfrel; fold (n_func_related m8 e n) in nfrel.
+        unfold so_func_related in sofrel; unfold bits_proj in sofrel;
         rewrite (nf_params_not_changed m7 e v4 m8 shifter_operand) in sofrel;
           [clear nf | exact nf];
-        fold (so_proj m8 e) in sofrel; fold (so_func_related m8 e so) in sofrel.
+        fold (bits_proj m8 e shifter_operand) in sofrel; fold (so_func_related m8 e so) in sofrel.
         inv main_p ;[idtac | nod];
         rename H4 into zf, H7 into main_p, H3 into evs;
         apply Events.Eapp_E0_inv in evs; destruct evs; subst.
@@ -2753,26 +2132,26 @@ Proof.
           s1
           d Events.E0 m9 v5) in psrel;
         [idtac| exact dfrel | exact zf].
-        unfold sbit_func_related in sfrel; unfold S_proj in sfrel;   
+        unfold sbit_func_related in sfrel; unfold bit_proj in sfrel;   
         rewrite (zf_params_not_changed m8 e v5 m9 S) in sfrel;
           [idtac | exact zf];
-        fold (S_proj m9 e) in sfrel; fold (sbit_func_related m9 e sbit) in sfrel.
+        fold (bit_proj m9 e S) in sfrel; fold (sbit_func_related m9 e sbit) in sfrel.
         unfold cond_func_related in cfrel; unfold cond_proj in cfrel;
         rewrite (zf_params_not_changed m8 e v5 m9 adc_compcert_fixed.cond) in cfrel;
           [idtac | exact zf];
         fold (cond_proj m9 e) in cfrel; fold (cond_func_related m9 e cond) in cfrel.
-        unfold d_func_related in dfrel; unfold d_proj in dfrel;
+        unfold d_func_related in dfrel; unfold reg_proj in dfrel;
         rewrite (zf_params_not_changed m8 e v5 m9 adc_compcert_fixed.d) in dfrel;
           [idtac | exact zf];
-        fold (d_proj m9 e) in dfrel; fold (d_func_related m9 e d) in dfrel.
-        unfold n_func_related in nfrel; unfold n_proj in nfrel;
+        fold (reg_proj m9 e adc_compcert_fixed.d) in dfrel; fold (d_func_related m9 e d) in dfrel.
+        unfold n_func_related in nfrel; unfold reg_proj in nfrel;
         rewrite (zf_params_not_changed m8 e v5 m9 adc_compcert_fixed.n) in nfrel;
           [idtac | exact zf]; 
-        fold (n_proj m9 e) in nfrel; fold (n_func_related m9 e n) in nfrel.
-        unfold so_func_related in sofrel; unfold so_proj in sofrel;
+        fold (reg_proj m9 e adc_compcert_fixed.n) in nfrel; fold (n_func_related m9 e n) in nfrel.
+        unfold so_func_related in sofrel; unfold bits_proj in sofrel;
         rewrite (zf_params_not_changed m8 e v5 m9 shifter_operand) in sofrel;
           [clear zf | exact zf];
-        fold (so_proj m9 e) in sofrel; fold (so_func_related m9 e so) in sofrel.
+        fold (bits_proj m9 e shifter_operand) in sofrel; fold (so_func_related m9 e so) in sofrel.
         inv main_p ;[idtac | nod];
         rename H4 into cf, H7 into vf, H3 into evs;
         apply Events.Eapp_E0_inv in evs; destruct evs; subst.
@@ -2786,26 +2165,26 @@ Proof.
           s s2
           n so Events.E0 m10 v6) in psrel;
         [idtac| exact nfrel | exact sofrel| exact cf]. 
-        unfold sbit_func_related in sfrel; unfold S_proj in sfrel;   
+        unfold sbit_func_related in sfrel; unfold bit_proj in sfrel;   
         rewrite (cf_params_not_changed m9 e v6 m10 S) in sfrel;
           [idtac | exact cf];
-        fold (S_proj m10 e) in sfrel; fold (sbit_func_related m10 e sbit) in sfrel.
+        fold (bit_proj m10 e S) in sfrel; fold (sbit_func_related m10 e sbit) in sfrel.
         unfold cond_func_related in cfrel; unfold cond_proj in cfrel;
         rewrite (cf_params_not_changed m9 e v6 m10 adc_compcert_fixed.cond) in cfrel;
           [idtac | exact cf];
         fold (cond_proj m10 e) in cfrel; fold (cond_func_related m10 e cond) in cfrel.
-        unfold d_func_related in dfrel; unfold d_proj in dfrel;
+        unfold d_func_related in dfrel; unfold reg_proj in dfrel;
         rewrite (cf_params_not_changed m9 e v6 m10 adc_compcert_fixed.d) in dfrel;
           [idtac | exact cf];
-        fold (d_proj m10 e) in dfrel; fold (d_func_related m10 e d) in dfrel.
-        unfold n_func_related in nfrel; unfold n_proj in nfrel;
+        fold (reg_proj m10 e adc_compcert_fixed.d) in dfrel; fold (d_func_related m10 e d) in dfrel.
+        unfold n_func_related in nfrel; unfold reg_proj in nfrel;
         rewrite (cf_params_not_changed m9 e v6 m10 adc_compcert_fixed.n) in nfrel;
           [idtac | exact cf]; 
-        fold (n_proj m10 e) in nfrel; fold (n_func_related m10 e n) in nfrel.
-        unfold so_func_related in sofrel; unfold so_proj in sofrel;
+        fold (reg_proj m10 e adc_compcert_fixed.n) in nfrel; fold (n_func_related m10 e n) in nfrel.
+        unfold so_func_related in sofrel; unfold bits_proj in sofrel;
         rewrite (cf_params_not_changed m9 e v6 m10 shifter_operand) in sofrel;
           [clear cf | exact cf];
-        fold (so_proj m10 e) in sofrel; fold (so_func_related m10 e so) in sofrel.
+        fold (bits_proj m10 e shifter_operand) in sofrel; fold (so_func_related m10 e so) in sofrel.
 
         unfold st in psrel.
         inv vf; rename H2 into vf;
@@ -2886,12 +2265,12 @@ Proof.
         unfold _set_bo at 1. unfold ok_semstate.
         unfold bind at 2.
         unfold bind at 1. unfold loc. unfold bo. unfold st. simpl.
-        simpl. rewrite same_bool. exact psrel.
+        simpl. rewrite same_bool. exact psrel. (*exact condpass0. exact condpass0.*)
 
     (* ConditionPassed(&proc->cpsr, cond) evaluates to false *)
     inv main_p.
     unfold S.ADC_step; unfold _get_st; unfold bind_s; unfold bind; simpl.
-    rewrite (condpass_false e mfin Events.E0 mfin v1); [simpl | inv cp_b|exact cp_b].
-    exact psrel.
+    rewrite (condpass_false m0 m1 e mfin Events.E0 mfin v1);
+      [simpl;exact psrel |exact al| exact condpass0 |exact cp_b].
 Qed.
 
