devel/xiaomu/projection.v
@@ -1,0 +1,733 @@
+(* This file describe the relation between COQ and C state for ARM *)
+
+Require Import Globalenvs Memory.
+Require Import Csyntax Csem Cstrategy Coqlib Integers Values Maps Errors. 
+Require Import Arm6_State Arm6_Proc Arm6_SCC Bitvec Arm6.
+Require Import adc_compcert_fixed.
+
+(* Some constants for ADC *)
+
+(* Initial local environment, an empty PTree contents var location & type*)
+Definition env0 := (PTree.empty (block * type)).
+
+(* Initialize the memory with program p defined in adc_compcert*)
+Definition mem0 := Genv.init_mem p. 
+
+(* If an option val is Some integer then return the integer value else return zero*)
+Definition load_val (v : option val):word:=
+  match v with
+    |Some (Vint v')=> v'                     
+    |_ => Int.zero
+  end.
+
+(* Find the offset for elements in a struct*)
+(* If there is no variable id in struct t then the returned offset will be zero
+   (this location is then the same as for t);
+   later, if you want to L/S a value from this location, it will return None
+ *)
+
+Definition ofs_of_fld (f_id:AST.ident) (fl:fieldlist) :word:=
+  match field_offset f_id fl with
+    | Error _ => Int.zero
+    | OK r => repr r
+  end.
+
+(* offset of each element in Processor Tstruct *)
+Definition cpsr_ofs:int:=ofs_of_fld cpsr typ_struct_SLv6_Processor.
+
+Definition spsr_ofs:int:=ofs_of_fld spsrs typ_struct_SLv6_Processor.
+
+Definition mode_ofs:int:=
+  add (ofs_of_fld cpsr typ_struct_SLv6_Processor) 
+  (ofs_of_fld mode typ_struct_SLv6_StatusRegister).
+
+Definition reg_ofs (id:AST.ident):int:=
+  ofs_of_fld id typ_struct_SLv6_Processor.
+
+Definition mmu_ofs:int:=ofs_of_fld mmu_ptr typ_struct_SLv6_Processor.
+
+Definition mem_ofs:int:=ofs_of_fld mem typ_struct_SLv6_MMU.
+
+Definition cp15_ofs:int:=ofs_of_fld cp15 typ_struct_SLv6_Processor.
+
+Definition pc_ofs:int:=ofs_of_fld pc typ_struct_SLv6_Processor.
+
+Definition id_ofs:int:=ofs_of_fld id typ_struct_SLv6_Processor.
+
+Definition jump_ofs:int:=ofs_of_fld jump typ_struct_SLv6_Processor.
+
+Definition proc_loc (m:Mem.mem) (e:env):option val:=
+  match e!proc with
+    |Some(b,_)=>
+      match 
+        (load_value_of_type (Tpointer typ_SLv6_Processor) m b Int.zero) with
+        |Some(Vptr b o) as v=>v
+        |_=>None
+      end
+    |None=>None
+  end.
+
+
+(* Projection from C parameters to COQ parameters*)
+(* If in local env the parameter of ADC (S, cond, d or n) exists,
+   then return the value of it else return zero*)
+
+Definition param_val (id:AST.ident) (m:Mem.mem) (e:env):val:=
+  match e!id with
+    |Some(b,t)=>
+      let ov:=load_value_of_type t m b Int.zero in
+        match ov with
+          |Some v=>v
+          |None=>Vundef
+        end
+    |None=>Vundef
+  end.
+
+Definition varg_proj (v:val):int:=
+  match v with
+    |Vint v'=>v'
+    |_=>Int.zero
+  end.
+
+(* singal bit parameter projection *)
+Definition bit_proj (m:Mem.mem) (e:env) (id:AST.ident):bool:=
+  eq (varg_proj (param_val id m e)) w1.
+
+(* condition parameter projection *)
+Definition cond_proj (m:Mem.mem) (e:env):opcode:= 
+  let c:=condition (varg_proj (param_val cond m e)) in
+    match c with
+      |Some c'=>c'
+      |None=>AL
+    end.
+
+(* register parameter projection *)
+Definition reg_proj (m:Mem.mem) (e:env) (id:AST.ident):regnum:=
+  mk_regnum (varg_proj (param_val id m e)).
+
+(* bits parameter projection*)
+Definition bits_proj (m:Mem.mem) (e:env) (id:AST.ident):word:=
+  varg_proj (param_val shifter_operand m e).
+
+
+Definition find_field (ofs:int) (m:Mem.mem) (e:env)
+  :option val:=
+  match proc_loc m e with
+    |Some(Vptr b o) => Some (Vptr b (add o ofs))
+    |_=>None
+  end.
+
+Definition find_cpsr (m:Mem.mem) (e:env):option val:=
+  find_field cpsr_ofs m e.
+
+Definition find_spsr (m:Mem.mem) (e:env):option val:=
+  find_field spsr_ofs m e.
+
+Definition find_reg (m:Mem.mem) (e:env) (rid:AST.ident):option val:=
+  find_field (ofs_of_fld rid typ_struct_SLv6_Processor) m e.
+
+Definition find_cp15 (m:Mem.mem) (e:env):option val:=
+  find_field cp15_ofs m e.
+
+Definition find_id (m:Mem.mem) (e:env):option val:=
+  find_field id_ofs m e.
+
+Definition find_jump (m:Mem.mem) (e:env):option val:=
+  find_field jump_ofs m e.
+
+(* If cpsr can be found, use the location of [cpsr] and the offset of 
+   mode in StatusRegister struct to get location of [mode]*)
+(* The mode field in cpsr and spsr should be the same. 
+   And the element of spsrs array which is in use should correspond to the same mode.
+   And the register array in use, should also corresponds to this mode.*)
+Definition find_mode (m:Mem.mem) (e:env):option val:=
+  match find_cpsr m e with
+    |Some(Vptr b ofs)=>Some(Vptr b (add ofs mode_ofs))
+    |_=>None
+  end.
+
+(* If in local environment the variable [porc] exists,
+   then return the pointer of [proc] field [mmu_ptr].
+   From this MMU struct, returns the pointer to the field [mem]*)
+Definition find_mmu (m:Mem.mem) (e:env):option val:=
+  match proc_loc m e with
+    |Some(Vptr bp op)=>
+      match 
+        (load_value_of_type (Tpointer typ_SLv6_MMU) m bp (add op mmu_ofs)) with
+        |Some(Vptr bm om) as v=>v
+        |_=>None
+      end
+    |_=>None
+  end.
+
+Definition find_mem (m:Mem.mem) (e:env):option val:=
+  match find_mmu m e with
+    |Some(Vptr bm om)=>
+      match 
+        (load_value_of_type (Tpointer(Tint I8 Unsigned)) m bm (add om mem_ofs)) with
+        |Some(Vptr b o) as v=>v
+        |_=>None
+      end
+    |_=>None
+  end.
+
+(* If in local environment the variable [proc] exists
+   then return the pointer of [proc] field [pc]*)
+(* the pointer to [pc] should point to the exact location of
+   the 16th element in array [user_regs]*)
+Definition find_pc (m:Mem.mem) (e:env):option val:=
+  match proc_loc m e with
+    |Some(Vptr b ofs)=>
+      match 
+        (load_value_of_type (Tpointer (Tint I32 Unsigned)) m b ofs) with
+        |Some(Vptr b o) as v=>v
+        |_=>None
+      end
+    |_=>None
+  end.
+
+Definition pc_usereg15 (m:Mem.mem) (e:env):Prop:=
+  find_pc m e = find_reg m e user_regs.
+
+Definition find_fld (f: Mem.mem->env->option val) (fld:fieldlist)
+  (id:AST.ident) (m:Mem.mem) (e:env):
+  option val:=
+  match f m e with
+    |Some(Vptr bp op)=> 
+      Some(Vptr bp (add op (ofs_of_fld id fld)))
+    |_=>None
+  end.
+
+(*
+(*memory blocks of SystemCoproc*)
+(*Record sc_mem := mk_scm
+  {eeb: option val;
+    ub: option val;
+    vb: option val}.
+*)
+Record sc_mem := mk_scm
+  {eeb: val;
+    ub: val;
+    vb: val}.
+
+Definition slv6_sc (m:Mem.mem) (e:env):option sc_mem:=
+  let fld_v b o id:= Vptr b (add o (ofs_of_fld id typ_struct_SLv6_SystemCoproc))
+    in
+    match find_cp15 m e with
+      |Some(Vptr b o)=> 
+        Some(mk_scm (fld_v b o ee_bit) (fld_v b o u_bit) (fld_v b o v_bit))
+      |_=>None
+  end.
+
+(*memory blocks of StatusRegister*)
+(*Record sr_mem := mk_srm
+  {nf: option val;
+    zf: option val;
+    cf: option val;
+    vf: option val;
+    qf: option val;
+    jf: option val;
+    ge0: option val;
+    ge1: option val;
+    ge2: option val;
+    ge3: option val;
+    ef: option val;
+    af: option val;
+    i_f: option val;
+    ff: option val;
+    tf: option val;
+    md: option val;
+    bg: option val}.
+*)
+Record sr_mem := mk_srm
+  {nf: val;
+    zf: val;
+    cf: val;
+    vf: val;
+    qf: val;
+    jf: val;
+    ge0: val;
+    ge1: val;
+    ge2: val;
+    ge3: val;
+    ef: val;
+    af: val;
+    i_f: val;
+    ff: val;
+    tf: val;
+    md: val;
+    bg: val}.
+
+Definition slv6_cpsr (m:Mem.mem) (e:env):option sr_mem:=
+  let fld_v b o id:=Vptr b (add o (ofs_of_fld id typ_struct_SLv6_StatusRegister))
+    in
+    match find_cpsr m e with
+      |Some(Vptr b o)=>
+        Some(mk_srm (fld_v b o N_flag) (fld_v b o Z_flag) (fld_v b o C_flag) 
+          (fld_v b o V_flag) (fld_v b o Q_flag) (fld_v b o J_flag) 
+          (fld_v b o GE0) (fld_v b o GE1) (fld_v b o GE2) (fld_v b o GE3)
+          (fld_v b o E_flag) (fld_v b o A_flag) (fld_v b o I_flag) 
+          (fld_v b o F_flag) (fld_v b o T_flag) (fld_v b o mode) 
+          (fld_v b o background))
+    |_=>None
+    end.
+
+Definition mode2mode (pm:proc_mode) :=
+  match pm with
+    |usr|sys=>(user_regs,5)
+    |exn e=>match e with
+              |fiq=>(fiq_regs,0)
+              |irq=>(irq_regs,1)
+              |svc=>(svc_regs,2)
+              |abt=>(abt_regs,3)
+              |und=>(und_regs,4)
+            end
+  end.
+
+(*Definition find_spsr_m (m:Mem.mem) (e:env) (em:exn_mode):option val:=
+  let ofs o :=
+    add o (repr ((snd (mode2mode (exn em)))*sizeof typ_SLv6_StatusRegister)) in
+  match find_spsr m e with
+    |Some(Vptr b o)=>
+      Some (Vptr b (ofs o))
+    |_=>None
+  end.
+*)
+Definition find_spsr_m (m:Mem.mem) (e:env):option(exn_mode->val):=
+  let ofs o em:=
+    add o (repr ((snd (mode2mode (exn em)))*sizeof typ_SLv6_StatusRegister)) in
+  match find_spsr m e with
+    |Some(Vptr b o)=>
+      Some(fun em=>(Vptr b (ofs o em)))
+    |_=>None
+  end.
+
+Definition blk_spsr (m:Mem.mem) (e:env):=
+  let ofs o em:=
+    add o (repr ((snd (mode2mode (exn em)))*sizeof typ_SLv6_StatusRegister)) in
+  match find_spsr m e with
+    |Some(Vptr b o)=>
+      Some(fun em=>(b, (ofs o em)))
+    |_=>None
+  end.
+
+Definition slv6_spsr (m:Mem.mem) (e:env):option(exn_mode->sr_mem):=
+  let fld_v b o id:=Vptr b (add o (ofs_of_fld id typ_struct_SLv6_StatusRegister))
+    in
+    match blk_spsr m e with
+      |Some v=>
+        Some(fun em=>let (b,o):=v em in 
+          mk_srm (fld_v b o N_flag) (fld_v b o Z_flag) (fld_v b o C_flag) 
+          (fld_v b o V_flag) (fld_v b o Q_flag) (fld_v b o J_flag) 
+          (fld_v b o GE0) (fld_v b o GE1) (fld_v b o GE2) (fld_v b o GE3)
+          (fld_v b o E_flag) (fld_v b o A_flag) (fld_v b o I_flag) 
+          (fld_v b o F_flag) (fld_v b o T_flag) (fld_v b o mode) 
+          (fld_v b o background))
+      |_=>None
+    end.
+
+(*memory blocks of MMU*)
+Record mmu_mem := mk_mmum
+  {bgn: val;
+    sz: val;
+    ed: val;
+    mm: val}.
+
+(*Record mmu_mem := mk_mmum
+  {bgn: option val;
+    sz: option val;
+    ed: option val;
+    mm: option val}.
+*)
+
+Definition slv6_mmu (m:Mem.mem) (e:env):option mmu_mem:=
+  let fld_v b o id:=Vptr b (add o (ofs_of_fld id typ_struct_SLv6_MMU)) in
+  match find_mmu m e with
+    |Some(Vptr b o)=>
+      Some(mk_mmum (fld_v b o begin) (fld_v b o size) 
+                   (fld_v b o _end) (fld_v b o mem))
+    |_=>None
+  end.
+
+(*memory blocks of proc*)
+Record proc_mem := mk_pcm
+  {mmup: mmu_mem;
+    cpsr_m: sr_mem;
+    spsr_m: exn_mode->sr_mem;
+    sc: sc_mem;
+    id: val;
+    rg: register->val;
+    p: val;
+    jp: val}.
+
+Definition reg2reg (r:register):=
+  match r with
+    |R k=>(user_regs,k)
+    |R_svc k _=>(svc_regs,mk_regnum k)
+    |R_abt k _=>(abt_regs,mk_regnum k)
+    |R_und k _=>(und_regs,mk_regnum k)
+    |R_irq k _=>(irq_regs,mk_regnum k)
+    |R_fiq k _=>(fiq_regs,mk_regnum k)
+  end.
+
+Definition slv6_proc (m:Mem.mem) (e:env):option proc_mem:=
+  let fld_v b o i:=Vptr b (add o (ofs_of_fld i typ_struct_SLv6_Processor)) in
+  let fld_reg b o r:=
+    Vptr b (add o (ofs_of_fld (fst(reg2reg r)) 
+      typ_struct_SLv6_Processor)) in
+  let mm:=slv6_mmu m e in
+  let c:=slv6_cpsr m e in
+  let s:=slv6_spsr m e in
+  let sc:=slv6_sc m e in
+    match proc_loc m e with
+      |Some(Vptr b o)=>
+        match mm,c,(*fs,is,ss,abs,us,*)s,sc with
+          |Some vm,Some vc,(*Some vfs,Some vis,Some vss,Some vabs,Some vus,*)
+            Some vs,Some vsc =>
+            Some(mk_pcm vm vc (*vfs vis vss vabs vus*) vs vsc 
+              (fld_v b o adc_compcert_fixed.id) 
+              (fld_reg b o)
+              (fld_v b o pc)
+              (fld_v b o jump))
+          |_,_,_,_(*,_,_,_,_*)=>None
+        end
+      |_=>None
+    end.
+
+(* From a StateRegister Tstruct to word*)
+Definition sr_proj (m:Mem.mem) (sr:sr_mem) :option word:=
+  let valof ptr typ :=
+    match ptr with
+      |Vptr b o=>load_value_of_type typ m b o
+      |_=>None
+    end in
+    let setcpsr n ov ow :=
+      match ov, ow with
+        |Some(Vint v), Some w=>Some (set_bit n v w)
+        |_,_=>None
+      end in 
+    let setcpsrs n1 n2 ov ow :=
+      match ov, ow with
+        |Some(Vint v), Some w=>Some (set_bits n1 n2 v w)
+        |_,_=>None
+      end in 
+    (setcpsr Nbit (valof sr.(nf) (Tint I8 Unsigned))
+    (setcpsr Zbit (valof sr.(zf) (Tint I8 Unsigned))
+    (setcpsr Cbit (valof sr.(cf) (Tint I8 Unsigned))
+    (setcpsr Vbit (valof sr.(vf) (Tint I8 Unsigned))
+    (setcpsr Qbit (valof sr.(qf) (Tint I8 Unsigned))
+    (setcpsr Jbit (valof sr.(jf) (Tint I8 Unsigned))
+(* set bits 16 to 19 is set GEbits*)
+    (setcpsr 19%nat (valof sr.(ge3) (Tint I8 Unsigned))
+    (setcpsr 18%nat (valof sr.(ge2) (Tint I8 Unsigned))
+    (setcpsr 17%nat (valof sr.(ge1) (Tint I8 Unsigned))
+    (setcpsr 16%nat (valof sr.(ge0) (Tint I8 Unsigned))
+    (setcpsr Ebit (valof sr.(ef) (Tint I8 Unsigned))
+    (setcpsr Abit (valof sr.(af) (Tint I8 Unsigned))
+    (setcpsr Ibit (valof sr.(i_f) (Tint I8 Unsigned))
+    (setcpsr Fbit (valof sr.(ff) (Tint I8 Unsigned)) 
+    (setcpsr Tbit (valof sr.(tf) (Tint I8 Unsigned)) 
+(* set bits 0 to 4 is set Mbits*)
+    (setcpsrs 0%nat 4%nat (valof sr.(md) (Tint I32 Unsigned)) 
+      (Some Int.zero))))))))))))))))).
+
+(* Projection form C cpsr to COQ cpsr*)
+Definition cpsr_proj (m:Mem.mem) (c:sr_mem):option word:=
+  sr_proj m c.
+
+Definition spsr_proj (m:Mem.mem) (s:exn_mode->sr_mem) (em:exn_mode):word:=
+  let sr:=s em in
+    match sr_proj m sr with
+      |Some w=>w
+      |None=>repr 16
+    end.
+
+(* Projection from C mode in cpsr, to COQ mode*)
+Definition mode_proj (m:Mem.mem) (c:sr_mem) :option proc_mode:=
+  match c.(md) with
+    |Vptr b o=>
+      match load_value_of_type (Tint I32 Unsigned) m b o with
+        |Some(Vint v)=>proc_mode_of_word v
+        |_=>None
+      end
+    |_=>None
+  end.
+
+
+(* Projection from C reg to COQ reg*)
+Definition regs_proj (m:Mem.mem) (p:proc_mem) (r:register):word:=
+  let valof k:=
+    match p.(rg) r with
+      |Vptr b o=>load_value_of_type (Tint I32 Unsigned) m b (add o (repr k))
+      |_=>None
+    end in
+    let reg_val v :=
+    match v with
+      |Some(Vint v')=> v'
+      |_=>w0
+    end in
+    reg_val (valof (snd(reg2reg r))).
+
+
+(* Projection from C memory to COQ memory*)
+Definition mem_proj (m:Mem.mem) (mu:mmu_mem) (ad:address): word:=
+  match mu.(mm) with
+    |Vptr b o=>
+      match
+        load_value_of_type (Tint I8 Unsigned) m b (add o (word_of_address ad)) with
+        |Some(Vint v)=>v
+        |_=>w0
+      end
+    |_=>w0
+  end.
+
+(*Definition mem_proj (m:Mem.mem) (e:env) (ad:address):option word:=
+  match (find_mem m e) with
+    |Some(Vptr b o)=>
+      match load_value_of_type (Tint I8 Unsigned) m b 
+        (add o (word_of_address ad)) with
+        |Some(Vint v)=>Some v
+        |_=>None
+      end
+    |_=>None
+  end.*)
+
+(* Projection from C cp15 to COQ SCC register*)
+Definition screg_proj (m:Mem.mem) (sc:sc_mem) (r:regnum): word:=
+  let bit_val_e :=
+  match sc.(eeb) with
+    |Vptr b o=> load_value_of_type (Tint I8 Unsigned) m b o
+    |_=>None
+  end in
+  let bit_val_u :=
+  match sc.(ub) with
+    |Vptr b o=> load_value_of_type (Tint I8 Unsigned) m b o
+    |_=>None
+  end in
+  let bit_val_v :=
+  match sc.(vb) with
+    |Vptr b o=> load_value_of_type (Tint I8 Unsigned) m b o
+    |_=>None
+  end in  
+  let setscreg n ov ow :=
+    match ov, ow with
+      |Some(Vint v),w=>set_bit n v w
+      |_,_=>w0
+    end in
+    setscreg Vbit (bit_val_v) 
+    (setscreg Ubit (bit_val_u) 
+    (setscreg EEbit (bit_val_e) Int.zero)).  
+
+
+(* Projection from C proc to COQ state. exn in COQ proc state is assigned by
+   a nil exception list*)
+
+Definition proc_proj (m:Mem.mem) (e:env):option (Arm6_State.state):=
+  let mkpst ocpsr vspsr vreg omode:=
+    match ocpsr, omode with
+      |Some vcpsr, Some vmode=>
+        Some (Arm6_Proc.mk_state vcpsr vspsr vreg nil vmode)
+      |_,_ => None
+    end in
+    let mksst vscreg vmem := Arm6_SCC.mk_state vscreg vmem in
+      let mkst oproc vscc :=
+        match oproc with
+          |Some vproc=>Some (Arm6_State.mk_state vproc vscc)
+          |_=>None
+        end in
+        let opc := slv6_proc m e in
+        match opc with
+          |Some pc =>
+            mkst (mkpst (cpsr_proj m pc.(cpsr_m)) (spsr_proj m pc.(spsr_m)) 
+            (regs_proj m pc) 
+            (mode_proj m pc.(cpsr_m)))
+          (mksst (screg_proj m pc.(sc)) (mem_proj m pc.(mmup)))
+          |None=>None
+        end.
+*)
+
+
+(* From a StateRegister Tstruct to word*)
+(* Every bit is transformed from uint8 to one bit *)
+
+Definition fld_sr:= typ_struct_SLv6_StatusRegister.
+
+
+Definition sr_proj (m:Mem.mem) (b:block) (ofs:int) :word:=
+  let load_val_of id tp :=
+    load_val (load_value_of_type tp m b 
+      (add ofs (ofs_of_fld id fld_sr))) in
+  let nflag := load_val_of N_flag (Tint I8 Unsigned) in
+  let zflag := load_val_of Z_flag (Tint I8 Unsigned) in
+  let cflag := load_val_of C_flag (Tint I8 Unsigned) in
+  let vflag := load_val_of V_flag (Tint I8 Unsigned) in
+  let qflag := load_val_of Q_flag (Tint I8 Unsigned) in
+  let jflag := load_val_of J_flag (Tint I8 Unsigned) in
+  let ge0 := load_val_of GE0 (Tint I8 Unsigned) in
+  let ge1 := load_val_of GE1 (Tint I8 Unsigned) in
+  let ge2 := load_val_of GE2 (Tint I8 Unsigned) in
+  let ge3 := load_val_of GE3 (Tint I8 Unsigned) in
+  let eflag := load_val_of E_flag (Tint I8 Unsigned) in
+  let aflag := load_val_of A_flag (Tint I8 Unsigned) in
+  let iflag :=  load_val_of I_flag (Tint I8 Unsigned) in
+  let fflag := load_val_of F_flag (Tint I8 Unsigned) in
+  let tflag := load_val_of T_flag (Tint I8 Unsigned) in
+  let md := load_val_of mode (Tint I32 Unsigned) in
+(* according to P49,
+   Implementations must read reversed bits as 0 and ignore writes to them.
+   So no setting bits for the reversed bits*)
+  let bg := Int.zero in
+    (set_bit Nbit nflag
+    (set_bit Zbit zflag
+    (set_bit Cbit cflag
+    (set_bit Vbit vflag
+    (set_bit Qbit qflag
+    (set_bit Jbit jflag
+(* set bits 16 to 19 is set GEbits*)
+    (set_bit 19 ge3
+    (set_bit 18 ge2
+    (set_bit 17 ge1
+    (set_bit 16 ge0
+    (set_bit Ebit eflag
+    (set_bit Abit aflag
+    (set_bit Ibit iflag 
+    (set_bit Fbit fflag 
+    (set_bit Tbit tflag 
+(* set bits 0 to 4 is set Mbits*)
+    (set_bits 4 0 md Int.zero)))))))))))))))).
+
+(* Projection form C cpsr to COQ cpsr*)
+(* If the location of cpsr is found, then project C cpsr to a word
+   else return zero*)
+Definition cpsr_proj (m:Mem.mem) (e:env) :word:=
+  match find_cpsr m e with
+    |Some (Vptr b ofs) => sr_proj m b ofs
+    |_ => Int.zero
+  end.
+
+(* Projection from C spsr to COQ spsr*)
+(* If the location of spsr of specified exception mode is found, 
+   then project C cpsr to a word else return zero*)
+Definition spsr_proj (m:Mem.mem) (e:env) (em:exn_mode):word:=
+  let ofs o n:=add o (repr (n*sizeof typ_SLv6_StatusRegister)) in
+  match find_spsr m e with
+    |Some(Vptr b o)=>
+      match em with
+        |fiq=>sr_proj m b (ofs o 0)
+        |irq=>sr_proj m b (ofs o 1)
+        |svc=>sr_proj m b (ofs o 2)
+        |abt=>sr_proj m b (ofs o 3)
+        |und=>sr_proj m b (ofs o 4)
+      end
+    |_=>Int.zero
+  end.
+
+(* Projection from C mode in cpsr, to COQ mode*)
+(* If the location of mode is found, 
+   then project C mode to a proc_mode else return default user mode*)
+(* The mode in cpsr should indecate which spsr mode is and which kind of register
+   is used*)
+Definition mode_proj (m:Mem.mem) (e:env) :proc_mode:=
+  let om:=match find_mode m e with
+    |Some(Vptr b ofs)=>
+      proc_mode_of_word (load_val 
+        (load_value_of_type (Tint I32 Unsigned) m b ofs))
+    |_=>None
+  end
+  in 
+  match om with
+    |Some md=>md
+    |None=>usr
+  end.
+
+(* Projection from C reg to COQ reg*)
+(* If the location of reg is found, and by knowing which register mode
+   and which register number it is, return the value of this register.
+   else return zero*)
+Definition regs_proj (m:Mem.mem) (e:env) (r:register):word:=
+  let load_reg id n m e:=
+    match find_reg m e id with 
+    |Some(Vptr b ofs)=>
+      load_val (load_value_of_type 
+        (Tint I32 Unsigned) m b (add ofs (repr n))) 
+    |_=>Int.zero
+  end
+    in
+  match r with
+    | R k => load_reg user_regs k m e
+    | R_svc k _=> load_reg svc_regs k m e
+    | R_abt k _=> load_reg abt_regs k m e
+    | R_und k _=> load_reg und_regs k m e
+    | R_irq k _=> load_reg irq_regs k m e
+    | R_fiq k _=> load_reg fiq_regs k m e
+  end.
+
+(* Projection from C memory to COQ memory*)
+(* If the location of memory is found, using the address to
+   get the content of such memory block, else return zero*)
+Definition mem_proj (m:Mem.mem) (e:env) (ad:address):word:=
+  match find_mem m e with
+    |Some(Vptr b ofs)=>
+      load_val (load_value_of_type 
+        (Tint I8 Unsigned) m b (add ofs (word_of_address ad)))
+    |_=>Int.zero
+  end.
+
+(* Projection from C cp15 to COQ SCC register*)
+(* If the location of cp15 is found, 
+   get the value of ee_bit u_bit and v_bit to set the bits in
+   COQ SCC reg*)
+
+Definition fld_sc :=typ_struct_SLv6_SystemCoproc.
+
+Definition screg_proj (m:Mem.mem) (e:env) (r:regnum):word:=
+  match find_cp15 m e with
+    |Some(Vptr b ofs)=>
+      let regbit id:=
+        load_val (load_value_of_type (Tint I8 Unsigned) m b
+        (add ofs (ofs_of_fld id fld_sc))) in
+        let ee := regbit ee_bit in
+        let u := regbit u_bit in
+        let v := regbit v_bit in
+        set_bit Vbit v (set_bit Ubit u (set_bit EEbit ee Int.zero))
+    |_=>Int.zero
+  end.
+
+(* Projection from C proc to COQ state. exn in COQ proc state is assigned by
+   a nil exception list*)
+Definition proc_proj (m:Mem.mem) (e:env):Arm6_State.state:=
+  Arm6_State.mk_state 
+  (Arm6_Proc.mk_state (cpsr_proj m e) (spsr_proj m e) (regs_proj m e) nil (mode_proj m e))
+  (Arm6_SCC.mk_state (screg_proj m e) (mem_proj m e)).
+
+
+(* Stating theorems *)
+
+Require Import Arm6_Simul.
+Import I.
+Import Arm6_Functions.Semantics.
+
+(*Inductive proc_state_related : Mem.mem -> env -> @result unit -> Prop :=
+  |proc_state_related_ok : 
+    forall m e l b v, 
+      proc_proj m e = Some v ->
+      proc_state_related m e (Ok tt (mk_semstate l b v))
+  |state_not_ok: 
+    forall e m mes,
+      proc_proj m e = None ->
+      proc_state_related m e (Ko mes)
+  |state_todo: 
+    forall e m mes,
+      proc_proj m e = None ->
+      proc_state_related m e (Todo mes).*)
+
+Inductive proc_state_related : Mem.mem -> env -> @result unit -> Prop :=
+  |proc_state_related_ok : 
+    forall m e l b, proc_state_related m e (Ok tt (mk_semstate l b (proc_proj m e)))
+  |state_not_ok: forall e m mes, proc_state_related m e (Ko mes)
+  |state_todo: forall e m mes, proc_state_related m e (Todo mes).
+
+(* Functional relation between the C memory module which contains proc, 
+   and the COQ specification of Arm6 state *)
+(*Definition proc_state_func_related (m:Mem.mem) (e:env) (s:Arm6_State.state) :Prop:=
+  proc_proj m e = s.*)
